Cleanup

examples/insertion_sort_free.v
@@ -12,27 +12,27 @@ Inductive sll (x : ptr) (len : nat) (lo : nat) (hi : nat) (h : heap) : Prop :=
   (hi) == (0) /\ (len) == (0) /\ (lo) == (7) /\ h = empty
 | sll_2 of ~~ ((x) == (null)) of
   exists (len1 : nat) (v : nat) (hi1 : nat) (lo1 : nat) (nxt : ptr),
-  exists h_sll_nxtlen1lo1hi1_513,
-  (0) <= (len1) /\ (0) <= (v) /\ (hi) == ((if (hi1) <= (v) then v else hi1)) /\ (len) == ((1) + (len1)) /\ (lo) == ((if (v) <= (lo1) then v else lo1)) /\ (v) <= (7) /\ h = x :-> v \+ x .+ 1 :-> nxt \+ h_sll_nxtlen1lo1hi1_513 /\ sll nxt len1 lo1 hi1 h_sll_nxtlen1lo1hi1_513.
+  exists h_sll_nxtlen1lo1hi1_618,
+  (0) <= (len1) /\ (0) <= (v) /\ (hi) == ((if (hi1) <= (v) then v else hi1)) /\ (len) == ((1) + (len1)) /\ (lo) == ((if (v) <= (lo1) then v else lo1)) /\ (v) <= (7) /\ h = x :-> v \+ x .+ 1 :-> nxt \+ h_sll_nxtlen1lo1hi1_618 /\ sll nxt len1 lo1 hi1 h_sll_nxtlen1lo1hi1_618.
 
 Inductive srtl (x : ptr) (len : nat) (lo : nat) (hi : nat) (h : heap) : Prop :=
 | srtl_1 of (x) == (null) of
   (hi) == (0) /\ (len) == (0) /\ (lo) == (7) /\ h = empty
 | srtl_2 of ~~ ((x) == (null)) of
   exists (len1 : nat) (v : nat) (hi1 : nat) (lo1 : nat) (nxt : ptr),
-  exists h_srtl_nxtlen1lo1hi1_514,
-  (0) <= (len1) /\ (0) <= (v) /\ (hi) == ((if (hi1) <= (v) then v else hi1)) /\ (len) == ((1) + (len1)) /\ (lo) == ((if (v) <= (lo1) then v else lo1)) /\ (v) <= (7) /\ (v) <= (lo1) /\ h = x :-> v \+ x .+ 1 :-> nxt \+ h_srtl_nxtlen1lo1hi1_514 /\ srtl nxt len1 lo1 hi1 h_srtl_nxtlen1lo1hi1_514.
+  exists h_srtl_nxtlen1lo1hi1_619,
+  (0) <= (len1) /\ (0) <= (v) /\ (hi) == ((if (hi1) <= (v) then v else hi1)) /\ (len) == ((1) + (len1)) /\ (lo) == ((if (v) <= (lo1) then v else lo1)) /\ (v) <= (7) /\ (v) <= (lo1) /\ h = x :-> v \+ x .+ 1 :-> nxt \+ h_srtl_nxtlen1lo1hi1_619 /\ srtl nxt len1 lo1 hi1 h_srtl_nxtlen1lo1hi1_619.
 
-Lemma pure1 : (0) == (0). Admitted.
-Hint Resolve pure1: ssl_pure.
-Lemma pure2 : (7) == (7). Admitted.
-Hint Resolve pure2: ssl_pure.
-Lemma pure3 hi1x vx2 : (0) <= (vx2) -> (vx2) <= (7) -> ((if (hi1x) <= (vx2) then vx2 else hi1x)) == ((if (hi1x) <= (vx2) then vx2 else hi1x)). Admitted.
-Hint Resolve pure3: ssl_pure.
-Lemma pure4 vx2 lo1x : (0) <= (vx2) -> (vx2) <= (7) -> ((if (vx2) <= (lo1x) then vx2 else lo1x)) == ((if (vx2) <= (lo1x) then vx2 else lo1x)). Admitted.
-Hint Resolve pure4: ssl_pure.
-Lemma pure5 len1x : (0) <= ((1) + (len1x)) -> (0) <= (len1x) -> ((1) + (len1x)) == ((1) + (len1x)). Admitted.
-Hint Resolve pure5: ssl_pure.
+Lemma pure128 : (0) = (0). Admitted.
+Hint Resolve pure128: ssl_pure.
+Lemma pure129 : (7) = (7). Admitted.
+Hint Resolve pure129: ssl_pure.
+Lemma pure130 hi1x vx2 : (vx2) <= (7) -> (0) <= (vx2) -> ((if (hi1x) <= (vx2) then vx2 else hi1x)) = ((if (hi1x) <= (vx2) then vx2 else hi1x)). Admitted.
+Hint Resolve pure130: ssl_pure.
+Lemma pure131 vx2 lo1x : (vx2) <= (7) -> (0) <= (vx2) -> ((if (vx2) <= (lo1x) then vx2 else lo1x)) = ((if (vx2) <= (lo1x) then vx2 else lo1x)). Admitted.
+Hint Resolve pure131: ssl_pure.
+Lemma pure132 len1x : (0) <= ((1) + (len1x)) -> (0) <= (len1x) -> ((1) + (len1x)) = ((1) + (len1x)). Admitted.
+Hint Resolve pure132: ssl_pure.
 
 Definition srtl_insert_type :=
   forall (vprogs : ptr * ptr),
@@ -41,14 +41,14 @@ Definition srtl_insert_type :=
     fun h =>
       let: (x, r) := vprogs in
       let: (k, n, lo, hi) := vghosts in
-      exists h_srtl_xnlohi_515,
-      (0) <= (k) /\ (0) <= (n) /\ (k) <= (7) /\ h = r :-> k \+ h_srtl_xnlohi_515 /\ srtl x n lo hi h_srtl_xnlohi_515,
+      exists h_srtl_xnlohi_620,
+      (0) <= (k) /\ (0) <= (n) /\ (k) <= (7) /\ h = r :-> k \+ h_srtl_xnlohi_620 /\ srtl x n lo hi h_srtl_xnlohi_620,
     [vfun (_: unit) h =>
       let: (x, r) := vprogs in
       let: (k, n, lo, hi) := vghosts in
       exists hi1 lo1 n1 y,
-      exists h_srtl_yn1lo1hi1_516,
-      (hi1) == ((if (hi) <= (k) then k else hi)) /\ (lo1) == ((if (k) <= (lo) then k else lo)) /\ (n1) == ((1) + (n)) /\ h = r :-> y \+ h_srtl_yn1lo1hi1_516 /\ srtl y n1 lo1 hi1 h_srtl_yn1lo1hi1_516
+      exists h_srtl_yn1lo1hi1_621,
+      (hi1) == ((if (hi) <= (k) then k else hi)) /\ (lo1) == ((if (k) <= (lo) then k else lo)) /\ (n1) == ((1) + (n)) /\ h = r :-> y \+ h_srtl_yn1lo1hi1_621 /\ srtl y n1 lo1 hi1 h_srtl_yn1lo1hi1_621
     ]).
 
 Variable srtl_insert : srtl_insert_type.
@@ -60,14 +60,14 @@ Definition insertion_sort_free_type :=
     fun h =>
       let: (x, r) := vprogs in
       let: (n, lo, hi) := vghosts in
-      exists h_sll_xnlohi_517,
-      (0) <= (n) /\ h = r :-> null \+ h_sll_xnlohi_517 /\ sll x n lo hi h_sll_xnlohi_517,
+      exists h_sll_xnlohi_622,
+      (0) <= (n) /\ h = r :-> null \+ h_sll_xnlohi_622 /\ sll x n lo hi h_sll_xnlohi_622,
     [vfun (_: unit) h =>
       let: (x, r) := vprogs in
       let: (n, lo, hi) := vghosts in
       exists y,
-      exists h_srtl_ynlohi_518,
-      h = r :-> y \+ h_srtl_ynlohi_518 /\ srtl y n lo hi h_srtl_ynlohi_518
+      exists h_srtl_ynlohi_623,
+      h = r :-> y \+ h_srtl_ynlohi_623 /\ srtl y n lo hi h_srtl_ynlohi_623
     ]).
 
 Program Definition insertion_sort_free : insertion_sort_free_type :=
@@ -93,115 +93,115 @@ Obligation Tactic := intro; move=>[x r]; ssl_program_simpl.
 Next Obligation.
 ssl_ghostelim_pre.
 move=>[[n lo] hi].
-ex_elim h_sll_xnlohi_517.
+ex_elim h_sll_xnlohi_622.
 move=>[phi_self0].
 move=>[sigma_self].
 subst h_self.
-move=>H_sll_xnlohi_517.
+move=>H_sll_xnlohi_622.
 ssl_ghostelim_post.
-ssl_open ((x) == (null)) H_sll_xnlohi_517.
-move=>[phi_sll_xnlohi_5170] [phi_sll_xnlohi_5171] [phi_sll_xnlohi_5172].
-move=>[sigma_sll_xnlohi_517].
-subst h_sll_xnlohi_517.
-try rename h_sll_xnlohi_517 into h_sll_xnlo_517.
-try rename H_sll_xnlohi_517 into H_sll_xnlo_517.
-try rename h_srtl_ynlohi_518 into h_srtl_ynlo_518.
-try rename H_srtl_ynlohi_518 into H_srtl_ynlo_518.
-try rename h_sll_xnlo_517 into h_sll_xn_517.
-try rename H_sll_xnlo_517 into H_sll_xn_517.
-try rename h_srtl_ynlo_518 into h_srtl_yn_518.
-try rename H_srtl_ynlo_518 into H_srtl_yn_518.
-try rename h_srtl_yn_518 into h_srtl_y_518.
-try rename H_srtl_yn_518 into H_srtl_y_518.
-try rename h_sll_xn_517 into h_sll_x_517.
-try rename H_sll_xn_517 into H_sll_x_517.
-try rename h_srtl_y_518 into h_srtl__518.
-try rename H_srtl_y_518 into H_srtl__518.
+ssl_open ((x) == (null)) H_sll_xnlohi_622.
+move=>[phi_sll_xnlohi_6220] [phi_sll_xnlohi_6221] [phi_sll_xnlohi_6222].
+move=>[sigma_sll_xnlohi_622].
+subst h_sll_xnlohi_622.
+try rename h_sll_xnlohi_622 into h_sll_xnlo_622.
+try rename H_sll_xnlohi_622 into H_sll_xnlo_622.
+try rename h_srtl_ynlohi_623 into h_srtl_ynlo_623.
+try rename H_srtl_ynlohi_623 into H_srtl_ynlo_623.
+try rename h_sll_xnlo_622 into h_sll_xn_622.
+try rename H_sll_xnlo_622 into H_sll_xn_622.
+try rename h_srtl_ynlo_623 into h_srtl_yn_623.
+try rename H_srtl_ynlo_623 into H_srtl_yn_623.
+try rename h_sll_xn_622 into h_sll_x_622.
+try rename H_sll_xn_622 into H_sll_x_622.
+try rename h_srtl_yn_623 into h_srtl_y_623.
+try rename H_srtl_yn_623 into H_srtl_y_623.
+try rename h_srtl_y_623 into h_srtl__623.
+try rename H_srtl_y_623 into H_srtl__623.
 ssl_emp;
 exists (null);
 exists (empty);
 sslauto.
-unfold_constructor 1;
+ssl_close 1;
 sslauto.
 ex_elim len1x vx hi1x lo1x nxtx.
-ex_elim h_sll_nxtxlen1xlo1xhi1x_513x.
-move=>[phi_sll_xnlohi_5170] [phi_sll_xnlohi_5171] [phi_sll_xnlohi_5172] [phi_sll_xnlohi_5173] [phi_sll_xnlohi_5174] [phi_sll_xnlohi_5175].
-move=>[sigma_sll_xnlohi_517].
-subst h_sll_xnlohi_517.
-move=>H_sll_nxtxlen1xlo1xhi1x_513x.
-try rename h_sll_xnlohi_517 into h_sll_xnlohi1xvxvxhi1x_517.
-try rename H_sll_xnlohi_517 into H_sll_xnlohi1xvxvxhi1x_517.
-try rename h_srtl_ynlohi_518 into h_srtl_ynlohi1xvxvxhi1x_518.
-try rename H_srtl_ynlohi_518 into H_srtl_ynlohi1xvxvxhi1x_518.
-try rename h_srtl_ynlohi1xvxvxhi1x_518 into h_srtl_ynvxlo1xvxlo1xhi1xvxvxhi1x_518.
-try rename H_srtl_ynlohi1xvxvxhi1x_518 into H_srtl_ynvxlo1xvxlo1xhi1xvxvxhi1x_518.
-try rename h_sll_xnlohi1xvxvxhi1x_517 into h_sll_xnvxlo1xvxlo1xhi1xvxvxhi1x_517.
-try rename H_sll_xnlohi1xvxvxhi1x_517 into H_sll_xnvxlo1xvxlo1xhi1xvxvxhi1x_517.
-try rename h_sll_xnvxlo1xvxlo1xhi1xvxvxhi1x_517 into h_sll_xlen1xvxlo1xvxlo1xhi1xvxvxhi1x_517.
-try rename H_sll_xnvxlo1xvxlo1xhi1xvxvxhi1x_517 into H_sll_xlen1xvxlo1xvxlo1xhi1xvxvxhi1x_517.
-try rename h_srtl_ynvxlo1xvxlo1xhi1xvxvxhi1x_518 into h_srtl_ylen1xvxlo1xvxlo1xhi1xvxvxhi1x_518.
-try rename H_srtl_ynvxlo1xvxlo1xhi1xvxvxhi1x_518 into H_srtl_ylen1xvxlo1xvxlo1xhi1xvxvxhi1x_518.
+ex_elim h_sll_nxtxlen1xlo1xhi1x_618x.
+move=>[phi_sll_xnlohi_6220] [phi_sll_xnlohi_6221] [phi_sll_xnlohi_6222] [phi_sll_xnlohi_6223] [phi_sll_xnlohi_6224] [phi_sll_xnlohi_6225].
+move=>[sigma_sll_xnlohi_622].
+subst h_sll_xnlohi_622.
+move=>H_sll_nxtxlen1xlo1xhi1x_618x.
+try rename h_sll_xnlohi_622 into h_sll_xnlohi1xvxvxhi1x_622.
+try rename H_sll_xnlohi_622 into H_sll_xnlohi1xvxvxhi1x_622.
+try rename h_srtl_ynlohi_623 into h_srtl_ynlohi1xvxvxhi1x_623.
+try rename H_srtl_ynlohi_623 into H_srtl_ynlohi1xvxvxhi1x_623.
+try rename h_sll_xnlohi1xvxvxhi1x_622 into h_sll_xnvxlo1xvxlo1xhi1xvxvxhi1x_622.
+try rename H_sll_xnlohi1xvxvxhi1x_622 into H_sll_xnvxlo1xvxlo1xhi1xvxvxhi1x_622.
+try rename h_srtl_ynlohi1xvxvxhi1x_623 into h_srtl_ynvxlo1xvxlo1xhi1xvxvxhi1x_623.
+try rename H_srtl_ynlohi1xvxvxhi1x_623 into H_srtl_ynvxlo1xvxlo1xhi1xvxvxhi1x_623.
+try rename h_sll_xnvxlo1xvxlo1xhi1xvxvxhi1x_622 into h_sll_xlen1xvxlo1xvxlo1xhi1xvxvxhi1x_622.
+try rename H_sll_xnvxlo1xvxlo1xhi1xvxvxhi1x_622 into H_sll_xlen1xvxlo1xvxlo1xhi1xvxvxhi1x_622.
+try rename h_srtl_ynvxlo1xvxlo1xhi1xvxvxhi1x_623 into h_srtl_ylen1xvxlo1xvxlo1xhi1xvxvxhi1x_623.
+try rename H_srtl_ynvxlo1xvxlo1xhi1xvxvxhi1x_623 into H_srtl_ylen1xvxlo1xvxlo1xhi1xvxvxhi1x_623.
 ssl_read x.
 try rename vx into vx2.
-try rename h_srtl_ylen1xvxlo1xvxlo1xhi1xvxvxhi1x_518 into h_srtl_ylen1xvx2lo1xvx2lo1xhi1xvx2vx2hi1x_518.
-try rename H_srtl_ylen1xvxlo1xvxlo1xhi1xvxvxhi1x_518 into H_srtl_ylen1xvx2lo1xvx2lo1xhi1xvx2vx2hi1x_518.
-try rename h_sll_xlen1xvxlo1xvxlo1xhi1xvxvxhi1x_517 into h_sll_xlen1xvx2lo1xvx2lo1xhi1xvx2vx2hi1x_517.
-try rename H_sll_xlen1xvxlo1xvxlo1xhi1xvxvxhi1x_517 into H_sll_xlen1xvx2lo1xvx2lo1xhi1xvx2vx2hi1x_517.
+try rename h_sll_xlen1xvxlo1xvxlo1xhi1xvxvxhi1x_622 into h_sll_xlen1xvx2lo1xvx2lo1xhi1xvx2vx2hi1x_622.
+try rename H_sll_xlen1xvxlo1xvxlo1xhi1xvxvxhi1x_622 into H_sll_xlen1xvx2lo1xvx2lo1xhi1xvx2vx2hi1x_622.
+try rename h_srtl_ylen1xvxlo1xvxlo1xhi1xvxvxhi1x_623 into h_srtl_ylen1xvx2lo1xvx2lo1xhi1xvx2vx2hi1x_623.
+try rename H_srtl_ylen1xvxlo1xvxlo1xhi1xvxvxhi1x_623 into H_srtl_ylen1xvx2lo1xvx2lo1xhi1xvx2vx2hi1x_623.
 ssl_read (x .+ 1).
 try rename nxtx into nxtx2.
-try rename h_sll_nxtxlen1xlo1xhi1x_513x into h_sll_nxtx2len1xlo1xhi1x_513x.
-try rename H_sll_nxtxlen1xlo1xhi1x_513x into H_sll_nxtx2len1xlo1xhi1x_513x.
-try rename h_sll_x1n1lo1hi1_5171 into h_sll_nxtx2len1xlo1xhi1x_513x.
-try rename H_sll_x1n1lo1hi1_5171 into H_sll_nxtx2len1xlo1xhi1x_513x.
-ssl_call_pre (r :-> null \+ h_sll_nxtx2len1xlo1xhi1x_513x).
+try rename h_sll_nxtxlen1xlo1xhi1x_618x into h_sll_nxtx2len1xlo1xhi1x_618x.
+try rename H_sll_nxtxlen1xlo1xhi1x_618x into H_sll_nxtx2len1xlo1xhi1x_618x.
+try rename h_sll_x1n1lo1hi1_6221 into h_sll_nxtx2len1xlo1xhi1x_618x.
+try rename H_sll_x1n1lo1hi1_6221 into H_sll_nxtx2len1xlo1xhi1x_618x.
+ssl_call_pre (r :-> null \+ h_sll_nxtx2len1xlo1xhi1x_618x).
 ssl_call (len1x, lo1x, hi1x).
-exists (h_sll_nxtx2len1xlo1xhi1x_513x);
+exists (h_sll_nxtx2len1xlo1xhi1x_618x);
 sslauto.
 ssl_frame_unfold.
 move=>h_call0.
 ex_elim y1.
-ex_elim h_srtl_y1len1xlo1xhi1x_5181.
+ex_elim h_srtl_y1len1xlo1xhi1x_6231.
 move=>[sigma_call0].
 subst h_call0.
-move=>H_srtl_y1len1xlo1xhi1x_5181.
+move=>H_srtl_y1len1xlo1xhi1x_6231.
 store_valid.
 ssl_read r.
 try rename y1 into y12.
-try rename h_srtl_y1len1xlo1xhi1x_5181 into h_srtl_y12len1xlo1xhi1x_5181.
-try rename H_srtl_y1len1xlo1xhi1x_5181 into H_srtl_y12len1xlo1xhi1x_5181.
-try rename h_srtl_x2n2lo2hi2_515 into h_srtl_y12len1xlo1xhi1x_5181.
-try rename H_srtl_x2n2lo2hi2_515 into H_srtl_y12len1xlo1xhi1x_5181.
+try rename h_srtl_y1len1xlo1xhi1x_6231 into h_srtl_y12len1xlo1xhi1x_6231.
+try rename H_srtl_y1len1xlo1xhi1x_6231 into H_srtl_y12len1xlo1xhi1x_6231.
+try rename h_srtl_x2n2lo2hi2_620 into h_srtl_y12len1xlo1xhi1x_6231.
+try rename H_srtl_x2n2lo2hi2_620 into H_srtl_y12len1xlo1xhi1x_6231.
 ssl_write r.
-ssl_call_pre (r :-> vx2 \+ h_srtl_y12len1xlo1xhi1x_5181).
+ssl_call_pre (r :-> vx2 \+ h_srtl_y12len1xlo1xhi1x_6231).
 ssl_call (vx2, len1x, lo1x, hi1x).
-exists (h_srtl_y12len1xlo1xhi1x_5181);
+exists (h_srtl_y12len1xlo1xhi1x_6231);
 sslauto.
 ssl_frame_unfold.
 move=>h_call1.
 ex_elim hi11 lo11 n11 y2.
-ex_elim h_srtl_y2n11lo11hi11_516.
+ex_elim h_srtl_y2n11lo11hi11_621.
 move=>[phi_call10] [phi_call11] [phi_call12].
 move=>[sigma_call1].
 subst h_call1.
-move=>H_srtl_y2n11lo11hi11_516.
+move=>H_srtl_y2n11lo11hi11_621.
 store_valid.
-try rename h_srtl_y2n11lo11hi11_516 into h_srtl_y2n11lo11hi1xvx2vx2hi1x_516.
-try rename H_srtl_y2n11lo11hi11_516 into H_srtl_y2n11lo11hi1xvx2vx2hi1x_516.
-try rename h_srtl_y2n11lo11hi1xvx2vx2hi1x_516 into h_srtl_y2n11vx2lo1xvx2lo1xhi1xvx2vx2hi1x_516.
-try rename H_srtl_y2n11lo11hi1xvx2vx2hi1x_516 into H_srtl_y2n11vx2lo1xvx2lo1xhi1xvx2vx2hi1x_516.
-try rename h_srtl_y2n11vx2lo1xvx2lo1xhi1xvx2vx2hi1x_516 into h_srtl_y2len1xvx2lo1xvx2lo1xhi1xvx2vx2hi1x_516.
-try rename H_srtl_y2n11vx2lo1xvx2lo1xhi1xvx2vx2hi1x_516 into H_srtl_y2len1xvx2lo1xvx2lo1xhi1xvx2vx2hi1x_516.
+try rename h_srtl_y2n11lo11hi11_621 into h_srtl_y2n11lo11hi1xvx2vx2hi1x_621.
+try rename H_srtl_y2n11lo11hi11_621 into H_srtl_y2n11lo11hi1xvx2vx2hi1x_621.
+try rename h_srtl_y2n11lo11hi1xvx2vx2hi1x_621 into h_srtl_y2n11vx2lo1xvx2lo1xhi1xvx2vx2hi1x_621.
+try rename H_srtl_y2n11lo11hi1xvx2vx2hi1x_621 into H_srtl_y2n11vx2lo1xvx2lo1xhi1xvx2vx2hi1x_621.
+try rename h_srtl_y2n11vx2lo1xvx2lo1xhi1xvx2vx2hi1x_621 into h_srtl_y2len1xvx2lo1xvx2lo1xhi1xvx2vx2hi1x_621.
+try rename H_srtl_y2n11vx2lo1xvx2lo1xhi1xvx2vx2hi1x_621 into H_srtl_y2len1xvx2lo1xvx2lo1xhi1xvx2vx2hi1x_621.
 ssl_read r.
 try rename y2 into y22.
-try rename h_srtl_y2len1xvx2lo1xvx2lo1xhi1xvx2vx2hi1x_516 into h_srtl_y22len1xvx2lo1xvx2lo1xhi1xvx2vx2hi1x_516.
-try rename H_srtl_y2len1xvx2lo1xvx2lo1xhi1xvx2vx2hi1x_516 into H_srtl_y22len1xvx2lo1xvx2lo1xhi1xvx2vx2hi1x_516.
-try rename h_srtl_ylen1xvx2lo1xvx2lo1xhi1xvx2vx2hi1x_518 into h_srtl_y22len1xvx2lo1xvx2lo1xhi1xvx2vx2hi1x_516.
-try rename H_srtl_ylen1xvx2lo1xvx2lo1xhi1xvx2vx2hi1x_518 into H_srtl_y22len1xvx2lo1xvx2lo1xhi1xvx2vx2hi1x_516.
+try rename h_srtl_y2len1xvx2lo1xvx2lo1xhi1xvx2vx2hi1x_621 into h_srtl_y22len1xvx2lo1xvx2lo1xhi1xvx2vx2hi1x_621.
+try rename H_srtl_y2len1xvx2lo1xvx2lo1xhi1xvx2vx2hi1x_621 into H_srtl_y22len1xvx2lo1xvx2lo1xhi1xvx2vx2hi1x_621.
+try rename h_srtl_ylen1xvx2lo1xvx2lo1xhi1xvx2vx2hi1x_623 into h_srtl_y22len1xvx2lo1xvx2lo1xhi1xvx2vx2hi1x_621.
+try rename H_srtl_ylen1xvx2lo1xvx2lo1xhi1xvx2vx2hi1x_623 into H_srtl_y22len1xvx2lo1xvx2lo1xhi1xvx2vx2hi1x_621.
 ssl_dealloc x.
 ssl_dealloc (x .+ 1).
 ssl_emp;
 exists (y22);
-exists (h_srtl_y22len1xvx2lo1xvx2lo1xhi1xvx2vx2hi1x_516);
+exists (h_srtl_y22len1xvx2lo1xvx2lo1xhi1xvx2vx2hi1x_621);
 sslauto.
 ssl_frame_unfold.
 Qed.
