examples/srtl_insert.v
@@ -12,53 +12,53 @@ Inductive sll (x : ptr) (len : nat) (lo : nat) (hi : nat) (h : heap) : Prop :=
   (hi) == (0) /\ (len) == (0) /\ (lo) == (7) /\ h = empty
 | sll_2 of ~~ ((x) == (null)) of
   exists (len1 : nat) (v : nat) (hi1 : nat) (lo1 : nat) (nxt : ptr),
-  exists h_sll_nxtlen1lo1hi1_519,
-  (0) <= (len1) /\ (0) <= (v) /\ (hi) == ((if (hi1) <= (v) then v else hi1)) /\ (len) == ((1) + (len1)) /\ (lo) == ((if (v) <= (lo1) then v else lo1)) /\ (v) <= (7) /\ h = x :-> v \+ x .+ 1 :-> nxt \+ h_sll_nxtlen1lo1hi1_519 /\ sll nxt len1 lo1 hi1 h_sll_nxtlen1lo1hi1_519.
+  exists h_sll_nxtlen1lo1hi1_624,
+  (0) <= (len1) /\ (0) <= (v) /\ (hi) == ((if (hi1) <= (v) then v else hi1)) /\ (len) == ((1) + (len1)) /\ (lo) == ((if (v) <= (lo1) then v else lo1)) /\ (v) <= (7) /\ h = x :-> v \+ x .+ 1 :-> nxt \+ h_sll_nxtlen1lo1hi1_624 /\ sll nxt len1 lo1 hi1 h_sll_nxtlen1lo1hi1_624.
 
 Inductive srtl (x : ptr) (len : nat) (lo : nat) (hi : nat) (h : heap) : Prop :=
 | srtl_1 of (x) == (null) of
   (hi) == (0) /\ (len) == (0) /\ (lo) == (7) /\ h = empty
 | srtl_2 of ~~ ((x) == (null)) of
   exists (len1 : nat) (v : nat) (hi1 : nat) (lo1 : nat) (nxt : ptr),
-  exists h_srtl_nxtlen1lo1hi1_520,
-  (0) <= (len1) /\ (0) <= (v) /\ (hi) == ((if (hi1) <= (v) then v else hi1)) /\ (len) == ((1) + (len1)) /\ (lo) == ((if (v) <= (lo1) then v else lo1)) /\ (v) <= (7) /\ (v) <= (lo1) /\ h = x :-> v \+ x .+ 1 :-> nxt \+ h_srtl_nxtlen1lo1hi1_520 /\ srtl nxt len1 lo1 hi1 h_srtl_nxtlen1lo1hi1_520.
+  exists h_srtl_nxtlen1lo1hi1_625,
+  (0) <= (len1) /\ (0) <= (v) /\ (hi) == ((if (hi1) <= (v) then v else hi1)) /\ (len) == ((1) + (len1)) /\ (lo) == ((if (v) <= (lo1) then v else lo1)) /\ (v) <= (7) /\ (v) <= (lo1) /\ h = x :-> v \+ x .+ 1 :-> nxt \+ h_srtl_nxtlen1lo1hi1_625 /\ srtl nxt len1 lo1 hi1 h_srtl_nxtlen1lo1hi1_625.
 
-Lemma pure6 : (0) <= (0). Admitted.
-Hint Resolve pure6: ssl_pure.
-Lemma pure7 : (1) == (1). Admitted.
-Hint Resolve pure7: ssl_pure.
-Lemma pure8 k2 : (k2) <= (7) -> (0) <= (k2) -> ((if (0) <= (k2) then k2 else 0)) == ((if (0) <= (k2) then k2 else 0)). Admitted.
-Hint Resolve pure8: ssl_pure.
-Lemma pure9 k2 : (k2) <= (7) -> (0) <= (k2) -> ((if (k2) <= (7) then k2 else 7)) == ((if (k2) <= (7) then k2 else 7)). Admitted.
-Hint Resolve pure9: ssl_pure.
-Lemma pure10 len1x : (0) <= ((1) + (len1x)) -> (0) <= (len1x) -> (((1) + (len1x)) + (1)) == ((1) + ((1) + (len1x))). Admitted.
-Hint Resolve pure10: ssl_pure.
-Lemma pure11 hi1x vx2 k2 lo1x : (vx2) <= (lo1x) -> (vx2) <= (k2) -> (0) <= (vx2) -> (k2) <= (vx2) -> (vx2) <= (7) -> (0) <= (k2) -> (k2) <= (7) -> ((if ((if (hi1x) <= (vx2) then vx2 else hi1x)) <= (k2) then k2 else (if (hi1x) <= (vx2) then vx2 else hi1x))) == ((if ((if (hi1x) <= (k2) then k2 else hi1x)) <= (vx2) then vx2 else (if (hi1x) <= (k2) then k2 else hi1x))). Admitted.
-Hint Resolve pure11: ssl_pure.
-Lemma pure12 vx2 k2 lo1x : (vx2) <= (lo1x) -> (vx2) <= (k2) -> (0) <= (vx2) -> (k2) <= (vx2) -> (vx2) <= (7) -> (0) <= (k2) -> (k2) <= (7) -> (vx2) <= ((if (k2) <= (lo1x) then k2 else lo1x)). Admitted.
-Hint Resolve pure12: ssl_pure.
-Lemma pure13 k2 vx2 lo1x : (vx2) <= (lo1x) -> (vx2) <= (k2) -> (0) <= (vx2) -> (k2) <= (vx2) -> (vx2) <= (7) -> (0) <= (k2) -> (k2) <= (7) -> ((if (k2) <= ((if (vx2) <= (lo1x) then vx2 else lo1x)) then k2 else (if (vx2) <= (lo1x) then vx2 else lo1x))) == ((if (vx2) <= ((if (k2) <= (lo1x) then k2 else lo1x)) then vx2 else (if (k2) <= (lo1x) then k2 else lo1x))). Admitted.
-Hint Resolve pure13: ssl_pure.
-Lemma pure14 k2 lo1x vx2 : (vx2) <= (lo1x) -> (vx2) <= (k2) -> (0) <= (vx2) -> (k2) <= (vx2) -> (vx2) <= (7) -> (0) <= (k2) -> (k2) <= (7) -> (k2) <= (lo1x). Admitted.
-Hint Resolve pure14: ssl_pure.
-Lemma pure15 len1x : (0) <= ((1) + (len1x)) -> (0) <= (len1x) -> (0) <= ((len1x) + (1)). Admitted.
-Hint Resolve pure15: ssl_pure.
-Lemma pure16 len1x : (0) <= ((1) + (len1x)) -> (0) <= (len1x) -> (((1) + (len1x)) + (1)) == ((1) + ((len1x) + (1))). Admitted.
-Hint Resolve pure16: ssl_pure.
-Lemma pure17 hi1x vx2 k2 lo1x : (vx2) <= (lo1x) -> (vx2) <= (k2) -> (0) <= (vx2) -> (~~ ((k2) <= (vx2))) || (~~ ((vx2) <= (k2))) -> (vx2) <= (7) -> (0) <= (k2) -> (k2) <= (7) -> ((if ((if (hi1x) <= (vx2) then vx2 else hi1x)) <= (k2) then k2 else (if (hi1x) <= (vx2) then vx2 else hi1x))) == ((if ((if (hi1x) <= (k2) then k2 else hi1x)) <= (vx2) then vx2 else (if (hi1x) <= (k2) then k2 else hi1x))). Admitted.
-Hint Resolve pure17: ssl_pure.
-Lemma pure18 vx2 k2 lo1x : (vx2) <= (lo1x) -> (vx2) <= (k2) -> (0) <= (vx2) -> (~~ ((k2) <= (vx2))) || (~~ ((vx2) <= (k2))) -> (vx2) <= (7) -> (0) <= (k2) -> (k2) <= (7) -> (vx2) <= ((if (k2) <= (lo1x) then k2 else lo1x)). Admitted.
-Hint Resolve pure18: ssl_pure.
-Lemma pure19 k2 vx2 lo1x : (vx2) <= (lo1x) -> (vx2) <= (k2) -> (0) <= (vx2) -> (~~ ((k2) <= (vx2))) || (~~ ((vx2) <= (k2))) -> (vx2) <= (7) -> (0) <= (k2) -> (k2) <= (7) -> ((if (k2) <= ((if (vx2) <= (lo1x) then vx2 else lo1x)) then k2 else (if (vx2) <= (lo1x) then vx2 else lo1x))) == ((if (vx2) <= ((if (k2) <= (lo1x) then k2 else lo1x)) then vx2 else (if (k2) <= (lo1x) then k2 else lo1x))). Admitted.
-Hint Resolve pure19: ssl_pure.
-Lemma pure20 len1x : (0) <= ((1) + (len1x)) -> (0) <= (len1x) -> (((1) + (len1x)) + (1)) == ((1) + ((1) + (len1x))). Admitted.
-Hint Resolve pure20: ssl_pure.
-Lemma pure21 hi1x vx2 k2 lo1x : (vx2) <= (lo1x) -> (0) <= (vx2) -> (vx2) <= (7) -> (0) <= (k2) -> ~~ ((vx2) <= (k2)) -> (k2) <= (7) -> ((if ((if (hi1x) <= (vx2) then vx2 else hi1x)) <= (k2) then k2 else (if (hi1x) <= (vx2) then vx2 else hi1x))) == ((if ((if (hi1x) <= (vx2) then vx2 else hi1x)) <= (k2) then k2 else (if (hi1x) <= (vx2) then vx2 else hi1x))). Admitted.
-Hint Resolve pure21: ssl_pure.
-Lemma pure22 k2 vx2 lo1x : (vx2) <= (lo1x) -> (0) <= (vx2) -> (vx2) <= (7) -> (0) <= (k2) -> ~~ ((vx2) <= (k2)) -> (k2) <= (7) -> (k2) <= ((if (vx2) <= (lo1x) then vx2 else lo1x)). Admitted.
-Hint Resolve pure22: ssl_pure.
-Lemma pure23 k2 vx2 lo1x : (vx2) <= (lo1x) -> (0) <= (vx2) -> (vx2) <= (7) -> (0) <= (k2) -> ~~ ((vx2) <= (k2)) -> (k2) <= (7) -> ((if (k2) <= ((if (vx2) <= (lo1x) then vx2 else lo1x)) then k2 else (if (vx2) <= (lo1x) then vx2 else lo1x))) == ((if (k2) <= ((if (vx2) <= (lo1x) then vx2 else lo1x)) then k2 else (if (vx2) <= (lo1x) then vx2 else lo1x))). Admitted.
-Hint Resolve pure23: ssl_pure.
+Lemma pure133 : (0) <= (0). Admitted.
+Hint Resolve pure133: ssl_pure.
+Lemma pure134 : (1) = (1). Admitted.
+Hint Resolve pure134: ssl_pure.
+Lemma pure135 k2 : (0) <= (k2) -> (k2) <= (7) -> ((if (0) <= (k2) then k2 else 0)) = ((if (0) <= (k2) then k2 else 0)). Admitted.
+Hint Resolve pure135: ssl_pure.
+Lemma pure136 k2 : (0) <= (k2) -> (k2) <= (7) -> ((if (k2) <= (7) then k2 else 7)) = ((if (k2) <= (7) then k2 else 7)). Admitted.
+Hint Resolve pure136: ssl_pure.
+Lemma pure137 len1x : (0) <= ((1) + (len1x)) -> (0) <= (len1x) -> (((1) + (len1x)) + (1)) = ((1) + ((1) + (len1x))). Admitted.
+Hint Resolve pure137: ssl_pure.
+Lemma pure138 k2 lo1x vx2 : (vx2) <= (lo1x) -> (vx2) <= (k2) -> (0) <= (vx2) -> (k2) <= (vx2) -> (vx2) <= (7) -> (0) <= (k2) -> (k2) <= (7) -> (k2) <= (lo1x). Admitted.
+Hint Resolve pure138: ssl_pure.
+Lemma pure139 hi1x vx2 k2 lo1x : (vx2) <= (lo1x) -> (vx2) <= (k2) -> (0) <= (vx2) -> (k2) <= (vx2) -> (vx2) <= (7) -> (0) <= (k2) -> (k2) <= (7) -> ((if ((if (hi1x) <= (vx2) then vx2 else hi1x)) <= (k2) then k2 else (if (hi1x) <= (vx2) then vx2 else hi1x))) = ((if ((if (hi1x) <= (k2) then k2 else hi1x)) <= (vx2) then vx2 else (if (hi1x) <= (k2) then k2 else hi1x))). Admitted.
+Hint Resolve pure139: ssl_pure.
+Lemma pure140 vx2 k2 lo1x : (vx2) <= (lo1x) -> (vx2) <= (k2) -> (0) <= (vx2) -> (k2) <= (vx2) -> (vx2) <= (7) -> (0) <= (k2) -> (k2) <= (7) -> (vx2) <= ((if (k2) <= (lo1x) then k2 else lo1x)). Admitted.
+Hint Resolve pure140: ssl_pure.
+Lemma pure141 k2 vx2 lo1x : (vx2) <= (lo1x) -> (vx2) <= (k2) -> (0) <= (vx2) -> (k2) <= (vx2) -> (vx2) <= (7) -> (0) <= (k2) -> (k2) <= (7) -> ((if (k2) <= ((if (vx2) <= (lo1x) then vx2 else lo1x)) then k2 else (if (vx2) <= (lo1x) then vx2 else lo1x))) = ((if (vx2) <= ((if (k2) <= (lo1x) then k2 else lo1x)) then vx2 else (if (k2) <= (lo1x) then k2 else lo1x))). Admitted.
+Hint Resolve pure141: ssl_pure.
+Lemma pure142 len1x : (0) <= ((1) + (len1x)) -> (0) <= (len1x) -> (0) <= ((len1x) + (1)). Admitted.
+Hint Resolve pure142: ssl_pure.
+Lemma pure143 len1x : (0) <= ((1) + (len1x)) -> (0) <= (len1x) -> (((1) + (len1x)) + (1)) = ((1) + ((len1x) + (1))). Admitted.
+Hint Resolve pure143: ssl_pure.
+Lemma pure144 hi1x vx2 k2 lo1x : (vx2) <= (lo1x) -> (vx2) <= (k2) -> (0) <= (vx2) -> (~~ ((k2) <= (vx2))) || (~~ ((vx2) <= (k2))) -> (vx2) <= (7) -> (0) <= (k2) -> (k2) <= (7) -> ((if ((if (hi1x) <= (vx2) then vx2 else hi1x)) <= (k2) then k2 else (if (hi1x) <= (vx2) then vx2 else hi1x))) = ((if ((if (hi1x) <= (k2) then k2 else hi1x)) <= (vx2) then vx2 else (if (hi1x) <= (k2) then k2 else hi1x))). Admitted.
+Hint Resolve pure144: ssl_pure.
+Lemma pure145 vx2 k2 lo1x : (vx2) <= (lo1x) -> (vx2) <= (k2) -> (0) <= (vx2) -> (~~ ((k2) <= (vx2))) || (~~ ((vx2) <= (k2))) -> (vx2) <= (7) -> (0) <= (k2) -> (k2) <= (7) -> (vx2) <= ((if (k2) <= (lo1x) then k2 else lo1x)). Admitted.
+Hint Resolve pure145: ssl_pure.
+Lemma pure146 k2 vx2 lo1x : (vx2) <= (lo1x) -> (vx2) <= (k2) -> (0) <= (vx2) -> (~~ ((k2) <= (vx2))) || (~~ ((vx2) <= (k2))) -> (vx2) <= (7) -> (0) <= (k2) -> (k2) <= (7) -> ((if (k2) <= ((if (vx2) <= (lo1x) then vx2 else lo1x)) then k2 else (if (vx2) <= (lo1x) then vx2 else lo1x))) = ((if (vx2) <= ((if (k2) <= (lo1x) then k2 else lo1x)) then vx2 else (if (k2) <= (lo1x) then k2 else lo1x))). Admitted.
+Hint Resolve pure146: ssl_pure.
+Lemma pure147 len1x : (0) <= ((1) + (len1x)) -> (0) <= (len1x) -> (((1) + (len1x)) + (1)) = ((1) + ((1) + (len1x))). Admitted.
+Hint Resolve pure147: ssl_pure.
+Lemma pure148 k2 vx2 lo1x : (vx2) <= (lo1x) -> (0) <= (vx2) -> (vx2) <= (7) -> (0) <= (k2) -> ~~ ((vx2) <= (k2)) -> (k2) <= (7) -> (k2) <= ((if (vx2) <= (lo1x) then vx2 else lo1x)). Admitted.
+Hint Resolve pure148: ssl_pure.
+Lemma pure149 k2 vx2 lo1x : (vx2) <= (lo1x) -> (0) <= (vx2) -> (vx2) <= (7) -> (0) <= (k2) -> ~~ ((vx2) <= (k2)) -> (k2) <= (7) -> ((if (k2) <= ((if (vx2) <= (lo1x) then vx2 else lo1x)) then k2 else (if (vx2) <= (lo1x) then vx2 else lo1x))) = ((if (k2) <= ((if (vx2) <= (lo1x) then vx2 else lo1x)) then k2 else (if (vx2) <= (lo1x) then vx2 else lo1x))). Admitted.
+Hint Resolve pure149: ssl_pure.
+Lemma pure150 hi1x vx2 k2 lo1x : (vx2) <= (lo1x) -> (0) <= (vx2) -> (vx2) <= (7) -> (0) <= (k2) -> ~~ ((vx2) <= (k2)) -> (k2) <= (7) -> ((if ((if (hi1x) <= (vx2) then vx2 else hi1x)) <= (k2) then k2 else (if (hi1x) <= (vx2) then vx2 else hi1x))) = ((if ((if (hi1x) <= (vx2) then vx2 else hi1x)) <= (k2) then k2 else (if (hi1x) <= (vx2) then vx2 else hi1x))). Admitted.
+Hint Resolve pure150: ssl_pure.
 
 Definition srtl_insert_type :=
   forall (vprogs : ptr * ptr),
@@ -67,14 +67,14 @@ Definition srtl_insert_type :=
     fun h =>
       let: (x, r) := vprogs in
       let: (k, n, lo, hi) := vghosts in
-      exists h_srtl_xnlohi_521,
-      (0) <= (k) /\ (0) <= (n) /\ (k) <= (7) /\ h = r :-> k \+ h_srtl_xnlohi_521 /\ srtl x n lo hi h_srtl_xnlohi_521,
+      exists h_srtl_xnlohi_626,
+      (0) <= (k) /\ (0) <= (n) /\ (k) <= (7) /\ h = r :-> k \+ h_srtl_xnlohi_626 /\ srtl x n lo hi h_srtl_xnlohi_626,
     [vfun (_: unit) h =>
       let: (x, r) := vprogs in
       let: (k, n, lo, hi) := vghosts in
       exists hi1 lo1 n1 y,
-      exists h_srtl_yn1lo1hi1_522,
-      (hi1) == ((if (hi) <= (k) then k else hi)) /\ (lo1) == ((if (k) <= (lo) then k else lo)) /\ (n1) == ((n) + (1)) /\ h = r :-> y \+ h_srtl_yn1lo1hi1_522 /\ srtl y n1 lo1 hi1 h_srtl_yn1lo1hi1_522
+      exists h_srtl_yn1lo1hi1_627,
+      (hi1) == ((if (hi) <= (k) then k else hi)) /\ (lo1) == ((if (k) <= (lo) then k else lo)) /\ (n1) == ((n) + (1)) /\ h = r :-> y \+ h_srtl_yn1lo1hi1_627 /\ srtl y n1 lo1 hi1 h_srtl_yn1lo1hi1_627
     ]).
 
 Program Definition srtl_insert : srtl_insert_type :=
@@ -123,50 +123,50 @@ Obligation Tactic := intro; move=>[x r]; ssl_program_simpl.
 Next Obligation.
 ssl_ghostelim_pre.
 move=>[[[k n] lo] hi].
-ex_elim h_srtl_xnlohi_521.
+ex_elim h_srtl_xnlohi_626.
 move=>[phi_self0] [phi_self1] [phi_self2].
 move=>[sigma_self].
 subst h_self.
-move=>H_srtl_xnlohi_521.
+move=>H_srtl_xnlohi_626.
 ssl_ghostelim_post.
-try rename h_srtl_yn1lo1hi1_522 into h_srtl_yn1lo1hikkhi_522.
-try rename H_srtl_yn1lo1hi1_522 into H_srtl_yn1lo1hikkhi_522.
-try rename h_srtl_yn1lo1hikkhi_522 into h_srtl_yn1kloklohikkhi_522.
-try rename H_srtl_yn1lo1hikkhi_522 into H_srtl_yn1kloklohikkhi_522.
-try rename h_srtl_yn1kloklohikkhi_522 into h_srtl_ynkloklohikkhi_522.
-try rename H_srtl_yn1kloklohikkhi_522 into H_srtl_ynkloklohikkhi_522.
+try rename h_srtl_yn1lo1hi1_627 into h_srtl_yn1lo1hikkhi_627.
+try rename H_srtl_yn1lo1hi1_627 into H_srtl_yn1lo1hikkhi_627.
+try rename h_srtl_yn1lo1hikkhi_627 into h_srtl_yn1kloklohikkhi_627.
+try rename H_srtl_yn1lo1hikkhi_627 into H_srtl_yn1kloklohikkhi_627.
+try rename h_srtl_yn1kloklohikkhi_627 into h_srtl_ynkloklohikkhi_627.
+try rename H_srtl_yn1kloklohikkhi_627 into H_srtl_ynkloklohikkhi_627.
 ssl_read r.
 try rename k into k2.
-try rename h_srtl_ynkloklohikkhi_522 into h_srtl_ynk2lok2lohik2k2hi_522.
-try rename H_srtl_ynkloklohikkhi_522 into H_srtl_ynk2lok2lohik2k2hi_522.
-ssl_open ((x) == (null)) H_srtl_xnlohi_521.
-move=>[phi_srtl_xnlohi_5210] [phi_srtl_xnlohi_5211] [phi_srtl_xnlohi_5212].
-move=>[sigma_srtl_xnlohi_521].
-subst h_srtl_xnlohi_521.
-try rename h_srtl_ynk2lok2lohik2k2hi_522 into h_srtl_ynk2lok2lok2k2_522.
-try rename H_srtl_ynk2lok2lohik2k2hi_522 into H_srtl_ynk2lok2lok2k2_522.
-try rename h_srtl_xnlohi_521 into h_srtl_xnlo_521.
-try rename H_srtl_xnlohi_521 into H_srtl_xnlo_521.
-try rename h_srtl_xnlo_521 into h_srtl_xn_521.
-try rename H_srtl_xnlo_521 into H_srtl_xn_521.
-try rename h_srtl_ynk2lok2lok2k2_522 into h_srtl_ynk2k2k2k2_522.
-try rename H_srtl_ynk2lok2lok2k2_522 into H_srtl_ynk2k2k2k2_522.
-try rename h_srtl_xn_521 into h_srtl_x_521.
-try rename H_srtl_xn_521 into H_srtl_x_521.
-try rename h_srtl_ynk2k2k2k2_522 into h_srtl_yk2k2k2k2_522.
-try rename H_srtl_ynk2k2k2k2_522 into H_srtl_yk2k2k2k2_522.
-try rename h_srtl_nxtylen1ylo11yhi11y_520y into h_srtl_nxtylen1ylo11y_520y.
-try rename H_srtl_nxtylen1ylo11yhi11y_520y into H_srtl_nxtylen1ylo11y_520y.
-try rename h_srtl_nxtylen1ylo11y_520y into h_srtl_nxtylo11y_520y.
-try rename H_srtl_nxtylen1ylo11y_520y into H_srtl_nxtylo11y_520y.
-try rename h_srtl_nxtylo11y_520y into h_srtl_nxty_520y.
-try rename H_srtl_nxtylo11y_520y into H_srtl_nxty_520y.
-try rename h_srtl_nxty_520y into h_srtl__520y.
-try rename H_srtl_nxty_520y into H_srtl__520y.
+try rename h_srtl_ynkloklohikkhi_627 into h_srtl_ynk2lok2lohik2k2hi_627.
+try rename H_srtl_ynkloklohikkhi_627 into H_srtl_ynk2lok2lohik2k2hi_627.
+ssl_open ((x) == (null)) H_srtl_xnlohi_626.
+move=>[phi_srtl_xnlohi_6260] [phi_srtl_xnlohi_6261] [phi_srtl_xnlohi_6262].
+move=>[sigma_srtl_xnlohi_626].
+subst h_srtl_xnlohi_626.
+try rename h_srtl_ynk2lok2lohik2k2hi_627 into h_srtl_ynk2lok2lok2k2_627.
+try rename H_srtl_ynk2lok2lohik2k2hi_627 into H_srtl_ynk2lok2lok2k2_627.
+try rename h_srtl_xnlohi_626 into h_srtl_xnlo_626.
+try rename H_srtl_xnlohi_626 into H_srtl_xnlo_626.
+try rename h_srtl_ynk2lok2lok2k2_627 into h_srtl_ynk2k2k2k2_627.
+try rename H_srtl_ynk2lok2lok2k2_627 into H_srtl_ynk2k2k2k2_627.
+try rename h_srtl_xnlo_626 into h_srtl_xn_626.
+try rename H_srtl_xnlo_626 into H_srtl_xn_626.
+try rename h_srtl_xn_626 into h_srtl_x_626.
+try rename H_srtl_xn_626 into H_srtl_x_626.
+try rename h_srtl_ynk2k2k2k2_627 into h_srtl_yk2k2k2k2_627.
+try rename H_srtl_ynk2k2k2k2_627 into H_srtl_yk2k2k2k2_627.
+try rename h_srtl_nxtylen1ylo11yhi11y_625y into h_srtl_nxtylen1ylo11y_625y.
+try rename H_srtl_nxtylen1ylo11yhi11y_625y into H_srtl_nxtylen1ylo11y_625y.
+try rename h_srtl_nxtylen1ylo11y_625y into h_srtl_nxtylo11y_625y.
+try rename H_srtl_nxtylen1ylo11y_625y into H_srtl_nxtylo11y_625y.
+try rename h_srtl_nxtylo11y_625y into h_srtl_nxty_625y.
+try rename H_srtl_nxtylo11y_625y into H_srtl_nxty_625y.
+try rename h_srtl_nxty_625y into h_srtl__625y.
+try rename H_srtl_nxty_625y into H_srtl__625y.
 ssl_alloc y2.
 try rename y into y2.
-try rename h_srtl_yk2k2k2k2_522 into h_srtl_y2k2k2k2k2_522.
-try rename H_srtl_yk2k2k2k2_522 into H_srtl_y2k2k2k2k2_522.
+try rename h_srtl_yk2k2k2k2_627 into h_srtl_y2k2k2k2k2_627.
+try rename H_srtl_yk2k2k2k2_627 into H_srtl_y2k2k2k2k2_627.
 ssl_write r.
 ssl_write_post r.
 ssl_write (y2 .+ 1).
@@ -177,172 +177,172 @@ ssl_emp;
 exists ((if (0) <= (k2) then k2 else 0)), ((if (k2) <= (7) then k2 else 7)), ((0) + (1)), (y2);
 exists (y2 :-> k2 \+ y2 .+ 1 :-> null);
 sslauto.
-unfold_constructor 2;
+ssl_close 2;
 exists (0), (k2), (0), (7), (null), (empty);
 sslauto.
-unfold_constructor 1;
+ssl_close 1;
 sslauto.
 ex_elim len1x vx hi1x lo1x nxtx.
-ex_elim h_srtl_nxtxlen1xlo1xhi1x_520x.
-move=>[phi_srtl_xnlohi_5210] [phi_srtl_xnlohi_5211] [phi_srtl_xnlohi_5212] [phi_srtl_xnlohi_5213] [phi_srtl_xnlohi_5214] [phi_srtl_xnlohi_5215] [phi_srtl_xnlohi_5216].
-move=>[sigma_srtl_xnlohi_521].
-subst h_srtl_xnlohi_521.
-move=>H_srtl_nxtxlen1xlo1xhi1x_520x.
-try rename h_srtl_ynk2lok2lohik2k2hi_522 into h_srtl_ynk2lok2lohi1xvxvxhi1xk2k2hi1xvxvxhi1x_522.
-try rename H_srtl_ynk2lok2lohik2k2hi_522 into H_srtl_ynk2lok2lohi1xvxvxhi1xk2k2hi1xvxvxhi1x_522.
-try rename h_srtl_xnlohi_521 into h_srtl_xnlohi1xvxvxhi1x_521.
-try rename H_srtl_xnlohi_521 into H_srtl_xnlohi1xvxvxhi1x_521.
-try rename h_srtl_xnlohi1xvxvxhi1x_521 into h_srtl_xnvxlo1xvxlo1xhi1xvxvxhi1x_521.
-try rename H_srtl_xnlohi1xvxvxhi1x_521 into H_srtl_xnvxlo1xvxlo1xhi1xvxvxhi1x_521.
-try rename h_srtl_ynk2lok2lohi1xvxvxhi1xk2k2hi1xvxvxhi1x_522 into h_srtl_ynk2vxlo1xvxlo1xk2vxlo1xvxlo1xhi1xvxvxhi1xk2k2hi1xvxvxhi1x_522.
-try rename H_srtl_ynk2lok2lohi1xvxvxhi1xk2k2hi1xvxvxhi1x_522 into H_srtl_ynk2vxlo1xvxlo1xk2vxlo1xvxlo1xhi1xvxvxhi1xk2k2hi1xvxvxhi1x_522.
-try rename h_srtl_ynk2vxlo1xvxlo1xk2vxlo1xvxlo1xhi1xvxvxhi1xk2k2hi1xvxvxhi1x_522 into h_srtl_ylen1xk2vxlo1xvxlo1xk2vxlo1xvxlo1xhi1xvxvxhi1xk2k2hi1xvxvxhi1x_522.
-try rename H_srtl_ynk2vxlo1xvxlo1xk2vxlo1xvxlo1xhi1xvxvxhi1xk2k2hi1xvxvxhi1x_522 into H_srtl_ylen1xk2vxlo1xvxlo1xk2vxlo1xvxlo1xhi1xvxvxhi1xk2k2hi1xvxvxhi1x_522.
-try rename h_srtl_xnvxlo1xvxlo1xhi1xvxvxhi1x_521 into h_srtl_xlen1xvxlo1xvxlo1xhi1xvxvxhi1x_521.
-try rename H_srtl_xnvxlo1xvxlo1xhi1xvxvxhi1x_521 into H_srtl_xlen1xvxlo1xvxlo1xhi1xvxvxhi1x_521.
+ex_elim h_srtl_nxtxlen1xlo1xhi1x_625x.
+move=>[phi_srtl_xnlohi_6260] [phi_srtl_xnlohi_6261] [phi_srtl_xnlohi_6262] [phi_srtl_xnlohi_6263] [phi_srtl_xnlohi_6264] [phi_srtl_xnlohi_6265] [phi_srtl_xnlohi_6266].
+move=>[sigma_srtl_xnlohi_626].
+subst h_srtl_xnlohi_626.
+move=>H_srtl_nxtxlen1xlo1xhi1x_625x.
+try rename h_srtl_ynk2lok2lohik2k2hi_627 into h_srtl_ynk2lok2lohi1xvxvxhi1xk2k2hi1xvxvxhi1x_627.
+try rename H_srtl_ynk2lok2lohik2k2hi_627 into H_srtl_ynk2lok2lohi1xvxvxhi1xk2k2hi1xvxvxhi1x_627.
+try rename h_srtl_xnlohi_626 into h_srtl_xnlohi1xvxvxhi1x_626.
+try rename H_srtl_xnlohi_626 into H_srtl_xnlohi1xvxvxhi1x_626.
+try rename h_srtl_ynk2lok2lohi1xvxvxhi1xk2k2hi1xvxvxhi1x_627 into h_srtl_ynk2vxlo1xvxlo1xk2vxlo1xvxlo1xhi1xvxvxhi1xk2k2hi1xvxvxhi1x_627.
+try rename H_srtl_ynk2lok2lohi1xvxvxhi1xk2k2hi1xvxvxhi1x_627 into H_srtl_ynk2vxlo1xvxlo1xk2vxlo1xvxlo1xhi1xvxvxhi1xk2k2hi1xvxvxhi1x_627.
+try rename h_srtl_xnlohi1xvxvxhi1x_626 into h_srtl_xnvxlo1xvxlo1xhi1xvxvxhi1x_626.
+try rename H_srtl_xnlohi1xvxvxhi1x_626 into H_srtl_xnvxlo1xvxlo1xhi1xvxvxhi1x_626.
+try rename h_srtl_ynk2vxlo1xvxlo1xk2vxlo1xvxlo1xhi1xvxvxhi1xk2k2hi1xvxvxhi1x_627 into h_srtl_ylen1xk2vxlo1xvxlo1xk2vxlo1xvxlo1xhi1xvxvxhi1xk2k2hi1xvxvxhi1x_627.
+try rename H_srtl_ynk2vxlo1xvxlo1xk2vxlo1xvxlo1xhi1xvxvxhi1xk2k2hi1xvxvxhi1x_627 into H_srtl_ylen1xk2vxlo1xvxlo1xk2vxlo1xvxlo1xhi1xvxvxhi1xk2k2hi1xvxvxhi1x_627.
+try rename h_srtl_xnvxlo1xvxlo1xhi1xvxvxhi1x_626 into h_srtl_xlen1xvxlo1xvxlo1xhi1xvxvxhi1x_626.
+try rename H_srtl_xnvxlo1xvxlo1xhi1xvxvxhi1x_626 into H_srtl_xlen1xvxlo1xvxlo1xhi1xvxvxhi1x_626.
 ssl_read x.
 try rename vx into vx2.
-try rename h_srtl_ylen1xk2vxlo1xvxlo1xk2vxlo1xvxlo1xhi1xvxvxhi1xk2k2hi1xvxvxhi1x_522 into h_srtl_ylen1xk2vx2lo1xvx2lo1xk2vx2lo1xvx2lo1xhi1xvx2vx2hi1xk2k2hi1xvx2vx2hi1x_522.
-try rename H_srtl_ylen1xk2vxlo1xvxlo1xk2vxlo1xvxlo1xhi1xvxvxhi1xk2k2hi1xvxvxhi1x_522 into H_srtl_ylen1xk2vx2lo1xvx2lo1xk2vx2lo1xvx2lo1xhi1xvx2vx2hi1xk2k2hi1xvx2vx2hi1x_522.
-try rename h_srtl_xlen1xvxlo1xvxlo1xhi1xvxvxhi1x_521 into h_srtl_xlen1xvx2lo1xvx2lo1xhi1xvx2vx2hi1x_521.
-try rename H_srtl_xlen1xvxlo1xvxlo1xhi1xvxvxhi1x_521 into H_srtl_xlen1xvx2lo1xvx2lo1xhi1xvx2vx2hi1x_521.
-ssl_abduce_branch (((k2) <= (vx2)) && ((vx2) <= (k2))).
+try rename h_srtl_xlen1xvxlo1xvxlo1xhi1xvxvxhi1x_626 into h_srtl_xlen1xvx2lo1xvx2lo1xhi1xvx2vx2hi1x_626.
+try rename H_srtl_xlen1xvxlo1xvxlo1xhi1xvxvxhi1x_626 into H_srtl_xlen1xvx2lo1xvx2lo1xhi1xvx2vx2hi1x_626.
+try rename h_srtl_ylen1xk2vxlo1xvxlo1xk2vxlo1xvxlo1xhi1xvxvxhi1xk2k2hi1xvxvxhi1x_627 into h_srtl_ylen1xk2vx2lo1xvx2lo1xk2vx2lo1xvx2lo1xhi1xvx2vx2hi1xk2k2hi1xvx2vx2hi1x_627.
+try rename H_srtl_ylen1xk2vxlo1xvxlo1xk2vxlo1xvxlo1xhi1xvxvxhi1xk2k2hi1xvxvxhi1x_627 into H_srtl_ylen1xk2vx2lo1xvx2lo1xk2vx2lo1xvx2lo1xhi1xvx2vx2hi1xk2k2hi1xvx2vx2hi1x_627.
+ssl_branch (((k2) <= (vx2)) && ((vx2) <= (k2))).
 ssl_read (x .+ 1).
 try rename nxtx into nxtx2.
-try rename h_srtl_nxtxlen1xlo1xhi1x_520x into h_srtl_nxtx2len1xlo1xhi1x_520x.
-try rename H_srtl_nxtxlen1xlo1xhi1x_520x into H_srtl_nxtx2len1xlo1xhi1x_520x.
-try rename h_srtl_nxtylen1ylo11yhi11y_520y into h_srtl_nxtylen1ylo11yhi11nxtyvnxtyvnxtyhi11nxty_520y.
-try rename H_srtl_nxtylen1ylo11yhi11y_520y into H_srtl_nxtylen1ylo11yhi11nxtyvnxtyvnxtyhi11nxty_520y.
-try rename h_srtl_nxtylen1ylo11yhi11nxtyvnxtyvnxtyhi11nxty_520y into h_srtl_nxtylen1nxtylo11yhi11nxtyvnxtyvnxtyhi11nxty_520y.
-try rename H_srtl_nxtylen1ylo11yhi11nxtyvnxtyvnxtyhi11nxty_520y into H_srtl_nxtylen1nxtylo11yhi11nxtyvnxtyvnxtyhi11nxty_520y.
-try rename h_srtl_nxtylen1nxtylo11yhi11nxtyvnxtyvnxtyhi11nxty_520y into h_srtl_nxtylen1nxtyvnxtylo11nxtyvnxtylo11nxtyhi11nxtyvnxtyvnxtyhi11nxty_520y.
-try rename H_srtl_nxtylen1nxtylo11yhi11nxtyvnxtyvnxtyhi11nxty_520y into H_srtl_nxtylen1nxtyvnxtylo11nxtyvnxtylo11nxtyhi11nxtyvnxtyvnxtyhi11nxty_520y.
-try rename h_srtl_nxtnxtylen1nxtylo11nxtyhi11nxty_520nxty into h_srtl_nxtx2len1xlo1xhi1x_520x.
-try rename H_srtl_nxtnxtylen1nxtylo11nxtyhi11nxty_520nxty into H_srtl_nxtx2len1xlo1xhi1x_520x.
-try rename h_srtl_nxtylen1nxtyvnxtylo11nxtyvnxtylo11nxtyhi11nxtyvnxtyvnxtyhi11nxty_520y into h_srtl_nxtylen1nxtyvnxtylo11nxtyvnxtylo11nxtyhi1xvnxtyvnxtyhi1x_520y.
-try rename H_srtl_nxtylen1nxtyvnxtylo11nxtyvnxtylo11nxtyhi11nxtyvnxtyvnxtyhi11nxty_520y into H_srtl_nxtylen1nxtyvnxtylo11nxtyvnxtylo11nxtyhi1xvnxtyvnxtyhi1x_520y.
-try rename h_srtl_nxtylen1nxtyvnxtylo11nxtyvnxtylo11nxtyhi1xvnxtyvnxtyhi1x_520y into h_srtl_nxtylen1xvnxtylo11nxtyvnxtylo11nxtyhi1xvnxtyvnxtyhi1x_520y.
-try rename H_srtl_nxtylen1nxtyvnxtylo11nxtyvnxtylo11nxtyhi1xvnxtyvnxtyhi1x_520y into H_srtl_nxtylen1xvnxtylo11nxtyvnxtylo11nxtyhi1xvnxtyvnxtyhi1x_520y.
-try rename h_srtl_nxtylen1xvnxtylo11nxtyvnxtylo11nxtyhi1xvnxtyvnxtyhi1x_520y into h_srtl_nxtylen1xvnxtylo1xvnxtylo1xhi1xvnxtyvnxtyhi1x_520y.
-try rename H_srtl_nxtylen1xvnxtylo11nxtyvnxtylo11nxtyhi1xvnxtyvnxtyhi1x_520y into H_srtl_nxtylen1xvnxtylo1xvnxtylo1xhi1xvnxtyvnxtyhi1x_520y.
-try rename h_srtl_ylen1xk2vx2lo1xvx2lo1xk2vx2lo1xvx2lo1xhi1xvx2vx2hi1xk2k2hi1xvx2vx2hi1x_522 into h_srtl_xlen1xk2vx2lo1xvx2lo1xk2vx2lo1xvx2lo1xhi1xvx2vx2hi1xk2k2hi1xvx2vx2hi1x_522.
-try rename H_srtl_ylen1xk2vx2lo1xvx2lo1xk2vx2lo1xvx2lo1xhi1xvx2vx2hi1xk2k2hi1xvx2vx2hi1x_522 into H_srtl_xlen1xk2vx2lo1xvx2lo1xk2vx2lo1xvx2lo1xhi1xvx2vx2hi1xk2k2hi1xvx2vx2hi1x_522.
+try rename h_srtl_nxtxlen1xlo1xhi1x_625x into h_srtl_nxtx2len1xlo1xhi1x_625x.
+try rename H_srtl_nxtxlen1xlo1xhi1x_625x into H_srtl_nxtx2len1xlo1xhi1x_625x.
+try rename h_srtl_nxtylen1ylo11yhi11y_625y into h_srtl_nxtylen1ylo11yhi11nxtyvnxtyvnxtyhi11nxty_625y.
+try rename H_srtl_nxtylen1ylo11yhi11y_625y into H_srtl_nxtylen1ylo11yhi11nxtyvnxtyvnxtyhi11nxty_625y.
+try rename h_srtl_nxtylen1ylo11yhi11nxtyvnxtyvnxtyhi11nxty_625y into h_srtl_nxtylen1nxtylo11yhi11nxtyvnxtyvnxtyhi11nxty_625y.
+try rename H_srtl_nxtylen1ylo11yhi11nxtyvnxtyvnxtyhi11nxty_625y into H_srtl_nxtylen1nxtylo11yhi11nxtyvnxtyvnxtyhi11nxty_625y.
+try rename h_srtl_nxtylen1nxtylo11yhi11nxtyvnxtyvnxtyhi11nxty_625y into h_srtl_nxtylen1nxtyvnxtylo11nxtyvnxtylo11nxtyhi11nxtyvnxtyvnxtyhi11nxty_625y.
+try rename H_srtl_nxtylen1nxtylo11yhi11nxtyvnxtyvnxtyhi11nxty_625y into H_srtl_nxtylen1nxtyvnxtylo11nxtyvnxtylo11nxtyhi11nxtyvnxtyvnxtyhi11nxty_625y.
+try rename h_srtl_nxtnxtylen1nxtylo11nxtyhi11nxty_625nxty into h_srtl_nxtx2len1xlo1xhi1x_625x.
+try rename H_srtl_nxtnxtylen1nxtylo11nxtyhi11nxty_625nxty into H_srtl_nxtx2len1xlo1xhi1x_625x.
+try rename h_srtl_nxtylen1nxtyvnxtylo11nxtyvnxtylo11nxtyhi11nxtyvnxtyvnxtyhi11nxty_625y into h_srtl_nxtylen1nxtyvnxtylo11nxtyvnxtylo11nxtyhi1xvnxtyvnxtyhi1x_625y.
+try rename H_srtl_nxtylen1nxtyvnxtylo11nxtyvnxtylo11nxtyhi11nxtyvnxtyvnxtyhi11nxty_625y into H_srtl_nxtylen1nxtyvnxtylo11nxtyvnxtylo11nxtyhi1xvnxtyvnxtyhi1x_625y.
+try rename h_srtl_nxtylen1nxtyvnxtylo11nxtyvnxtylo11nxtyhi1xvnxtyvnxtyhi1x_625y into h_srtl_nxtylen1xvnxtylo11nxtyvnxtylo11nxtyhi1xvnxtyvnxtyhi1x_625y.
+try rename H_srtl_nxtylen1nxtyvnxtylo11nxtyvnxtylo11nxtyhi1xvnxtyvnxtyhi1x_625y into H_srtl_nxtylen1xvnxtylo11nxtyvnxtylo11nxtyhi1xvnxtyvnxtyhi1x_625y.
+try rename h_srtl_nxtylen1xvnxtylo11nxtyvnxtylo11nxtyhi1xvnxtyvnxtyhi1x_625y into h_srtl_nxtylen1xvnxtylo1xvnxtylo1xhi1xvnxtyvnxtyhi1x_625y.
+try rename H_srtl_nxtylen1xvnxtylo11nxtyvnxtylo11nxtyhi1xvnxtyvnxtyhi1x_625y into H_srtl_nxtylen1xvnxtylo1xvnxtylo1xhi1xvnxtyvnxtyhi1x_625y.
+try rename h_srtl_ylen1xk2vx2lo1xvx2lo1xk2vx2lo1xvx2lo1xhi1xvx2vx2hi1xk2k2hi1xvx2vx2hi1x_627 into h_srtl_xlen1xk2vx2lo1xvx2lo1xk2vx2lo1xvx2lo1xhi1xvx2vx2hi1xk2k2hi1xvx2vx2hi1x_627.
+try rename H_srtl_ylen1xk2vx2lo1xvx2lo1xk2vx2lo1xvx2lo1xhi1xvx2vx2hi1xk2k2hi1xvx2vx2hi1x_627 into H_srtl_xlen1xk2vx2lo1xvx2lo1xk2vx2lo1xvx2lo1xhi1xvx2vx2hi1xk2k2hi1xvx2vx2hi1x_627.
 ssl_alloc nxty2.
 try rename nxty into nxty2.
-try rename h_srtl_nxtylen1xvnxtylo1xvnxtylo1xhi1xvnxtyvnxtyhi1x_520y into h_srtl_nxty2len1xvnxtylo1xvnxtylo1xhi1xvnxtyvnxtyhi1x_520y.
-try rename H_srtl_nxtylen1xvnxtylo1xvnxtylo1xhi1xvnxtyvnxtyhi1x_520y into H_srtl_nxty2len1xvnxtylo1xvnxtylo1xhi1xvnxtyvnxtyhi1x_520y.
+try rename h_srtl_nxtylen1xvnxtylo1xvnxtylo1xhi1xvnxtyvnxtyhi1x_625y into h_srtl_nxty2len1xvnxtylo1xvnxtylo1xhi1xvnxtyvnxtyhi1x_625y.
+try rename H_srtl_nxtylen1xvnxtylo1xvnxtylo1xhi1xvnxtyvnxtyhi1x_625y into H_srtl_nxty2len1xvnxtylo1xvnxtylo1xhi1xvnxtyvnxtyhi1x_625y.
 ssl_write (x .+ 1).
 ssl_write_post (x .+ 1).
 ssl_write r.
 ssl_write_post r.
 ssl_write (nxty2 .+ 1).
 ssl_write_post (nxty2 .+ 1).
-try rename h_srtl_nxty2len1xvnxtylo1xvnxtylo1xhi1xvnxtyvnxtyhi1x_520y into h_srtl_nxty2len1xk2lo1xk2lo1xhi1xk2k2hi1x_520y.
-try rename H_srtl_nxty2len1xvnxtylo1xvnxtylo1xhi1xvnxtyvnxtyhi1x_520y into H_srtl_nxty2len1xk2lo1xk2lo1xhi1xk2k2hi1x_520y.
+try rename h_srtl_nxty2len1xvnxtylo1xvnxtylo1xhi1xvnxtyvnxtyhi1x_625y into h_srtl_nxty2len1xk2lo1xk2lo1xhi1xk2k2hi1x_625y.
+try rename H_srtl_nxty2len1xvnxtylo1xvnxtylo1xhi1xvnxtyvnxtyhi1x_625y into H_srtl_nxty2len1xk2lo1xk2lo1xhi1xk2k2hi1x_625y.
 ssl_write nxty2.
 ssl_write_post nxty2.
 ssl_emp;
 exists ((if ((if (hi1x) <= (vx2) then vx2 else hi1x)) <= (k2) then k2 else (if (hi1x) <= (vx2) then vx2 else hi1x))), ((if (k2) <= ((if (vx2) <= (lo1x) then vx2 else lo1x)) then k2 else (if (vx2) <= (lo1x) then vx2 else lo1x))), (((1) + (len1x)) + (1)), (x);
-exists (x :-> vx2 \+ x .+ 1 :-> nxty2 \+ nxty2 :-> k2 \+ nxty2 .+ 1 :-> nxtx2 \+ h_srtl_nxtx2len1xlo1xhi1x_520x);
+exists (x :-> vx2 \+ x .+ 1 :-> nxty2 \+ nxty2 :-> k2 \+ nxty2 .+ 1 :-> nxtx2 \+ h_srtl_nxtx2len1xlo1xhi1x_625x);
 sslauto.
-unfold_constructor 2;
-exists ((1) + (len1x)), (vx2), ((if (hi1x) <= (k2) then k2 else hi1x)), ((if (k2) <= (lo1x) then k2 else lo1x)), (nxty2), (nxty2 :-> k2 \+ nxty2 .+ 1 :-> nxtx2 \+ h_srtl_nxtx2len1xlo1xhi1x_520x);
+ssl_close 2;
+exists ((1) + (len1x)), (vx2), ((if (hi1x) <= (k2) then k2 else hi1x)), ((if (k2) <= (lo1x) then k2 else lo1x)), (nxty2), (nxty2 :-> k2 \+ nxty2 .+ 1 :-> nxtx2 \+ h_srtl_nxtx2len1xlo1xhi1x_625x);
 sslauto.
-unfold_constructor 2;
-exists (len1x), (k2), (hi1x), (lo1x), (nxtx2), (h_srtl_nxtx2len1xlo1xhi1x_520x);
+ssl_close 2;
+exists (len1x), (k2), (hi1x), (lo1x), (nxtx2), (h_srtl_nxtx2len1xlo1xhi1x_625x);
 sslauto.
 ssl_frame_unfold.
-ssl_abduce_branch ((vx2) <= (k2)).
+ssl_branch ((vx2) <= (k2)).
 ssl_read (x .+ 1).
 try rename nxtx into nxtx2.
-try rename h_srtl_nxtxlen1xlo1xhi1x_520x into h_srtl_nxtx2len1xlo1xhi1x_520x.
-try rename H_srtl_nxtxlen1xlo1xhi1x_520x into H_srtl_nxtx2len1xlo1xhi1x_520x.
-try rename h_srtl_x1n2lo2hi2_5211 into h_srtl_nxtx2len1xlo1xhi1x_520x.
-try rename H_srtl_x1n2lo2hi2_5211 into H_srtl_nxtx2len1xlo1xhi1x_520x.
-ssl_call_pre (r :-> k2 \+ h_srtl_nxtx2len1xlo1xhi1x_520x).
+try rename h_srtl_nxtxlen1xlo1xhi1x_625x into h_srtl_nxtx2len1xlo1xhi1x_625x.
+try rename H_srtl_nxtxlen1xlo1xhi1x_625x into H_srtl_nxtx2len1xlo1xhi1x_625x.
+try rename h_srtl_x1n2lo2hi2_6261 into h_srtl_nxtx2len1xlo1xhi1x_625x.
+try rename H_srtl_x1n2lo2hi2_6261 into H_srtl_nxtx2len1xlo1xhi1x_625x.
+ssl_call_pre (r :-> k2 \+ h_srtl_nxtx2len1xlo1xhi1x_625x).
 ssl_call (k2, len1x, lo1x, hi1x).
-exists (h_srtl_nxtx2len1xlo1xhi1x_520x);
+exists (h_srtl_nxtx2len1xlo1xhi1x_625x);
 sslauto.
 ssl_frame_unfold.
 move=>h_call0.
 ex_elim hi11 lo11 n11 y1.
-ex_elim h_srtl_y1n11lo11hi11_5221.
+ex_elim h_srtl_y1n11lo11hi11_6271.
 move=>[phi_call00] [phi_call01] [phi_call02].
 move=>[sigma_call0].
 subst h_call0.
-move=>H_srtl_y1n11lo11hi11_5221.
+move=>H_srtl_y1n11lo11hi11_6271.
 store_valid.
-try rename h_srtl_y1n11lo11hi11_5221 into h_srtl_y1n11lo11hi1xk2k2hi1x_5221.
-try rename H_srtl_y1n11lo11hi11_5221 into H_srtl_y1n11lo11hi1xk2k2hi1x_5221.
-try rename h_srtl_y1n11lo11hi1xk2k2hi1x_5221 into h_srtl_y1n11k2lo1xk2lo1xhi1xk2k2hi1x_5221.
-try rename H_srtl_y1n11lo11hi1xk2k2hi1x_5221 into H_srtl_y1n11k2lo1xk2lo1xhi1xk2k2hi1x_5221.
-try rename h_srtl_y1n11k2lo1xk2lo1xhi1xk2k2hi1x_5221 into h_srtl_y1len1xk2lo1xk2lo1xhi1xk2k2hi1x_5221.
-try rename H_srtl_y1n11k2lo1xk2lo1xhi1xk2k2hi1x_5221 into H_srtl_y1len1xk2lo1xk2lo1xhi1xk2k2hi1x_5221.
+try rename h_srtl_y1n11lo11hi11_6271 into h_srtl_y1n11lo11hi1xk2k2hi1x_6271.
+try rename H_srtl_y1n11lo11hi11_6271 into H_srtl_y1n11lo11hi1xk2k2hi1x_6271.
+try rename h_srtl_y1n11lo11hi1xk2k2hi1x_6271 into h_srtl_y1n11k2lo1xk2lo1xhi1xk2k2hi1x_6271.
+try rename H_srtl_y1n11lo11hi1xk2k2hi1x_6271 into H_srtl_y1n11k2lo1xk2lo1xhi1xk2k2hi1x_6271.
+try rename h_srtl_y1n11k2lo1xk2lo1xhi1xk2k2hi1x_6271 into h_srtl_y1len1xk2lo1xk2lo1xhi1xk2k2hi1x_6271.
+try rename H_srtl_y1n11k2lo1xk2lo1xhi1xk2k2hi1x_6271 into H_srtl_y1len1xk2lo1xk2lo1xhi1xk2k2hi1x_6271.
 ssl_read r.
 try rename y1 into y12.
-try rename h_srtl_y1len1xk2lo1xk2lo1xhi1xk2k2hi1x_5221 into h_srtl_y12len1xk2lo1xk2lo1xhi1xk2k2hi1x_5221.
-try rename H_srtl_y1len1xk2lo1xk2lo1xhi1xk2k2hi1x_5221 into H_srtl_y12len1xk2lo1xk2lo1xhi1xk2k2hi1x_5221.
-try rename h_srtl_nxtylen1ylo12yhi12y_520y into h_srtl_y12len1xk2lo1xk2lo1xhi1xk2k2hi1x_5221.
-try rename H_srtl_nxtylen1ylo12yhi12y_520y into H_srtl_y12len1xk2lo1xk2lo1xhi1xk2k2hi1x_5221.
-try rename h_srtl_ylen1xk2vx2lo1xvx2lo1xk2vx2lo1xvx2lo1xhi1xvx2vx2hi1xk2k2hi1xvx2vx2hi1x_522 into h_srtl_xlen1xk2vx2lo1xvx2lo1xk2vx2lo1xvx2lo1xhi1xvx2vx2hi1xk2k2hi1xvx2vx2hi1x_522.
-try rename H_srtl_ylen1xk2vx2lo1xvx2lo1xk2vx2lo1xvx2lo1xhi1xvx2vx2hi1xk2k2hi1xvx2vx2hi1x_522 into H_srtl_xlen1xk2vx2lo1xvx2lo1xk2vx2lo1xvx2lo1xhi1xvx2vx2hi1xk2k2hi1xvx2vx2hi1x_522.
+try rename h_srtl_y1len1xk2lo1xk2lo1xhi1xk2k2hi1x_6271 into h_srtl_y12len1xk2lo1xk2lo1xhi1xk2k2hi1x_6271.
+try rename H_srtl_y1len1xk2lo1xk2lo1xhi1xk2k2hi1x_6271 into H_srtl_y12len1xk2lo1xk2lo1xhi1xk2k2hi1x_6271.
+try rename h_srtl_nxtylen1ylo12yhi12y_625y into h_srtl_y12len1xk2lo1xk2lo1xhi1xk2k2hi1x_6271.
+try rename H_srtl_nxtylen1ylo12yhi12y_625y into H_srtl_y12len1xk2lo1xk2lo1xhi1xk2k2hi1x_6271.
+try rename h_srtl_ylen1xk2vx2lo1xvx2lo1xk2vx2lo1xvx2lo1xhi1xvx2vx2hi1xk2k2hi1xvx2vx2hi1x_627 into h_srtl_xlen1xk2vx2lo1xvx2lo1xk2vx2lo1xvx2lo1xhi1xvx2vx2hi1xk2k2hi1xvx2vx2hi1x_627.
+try rename H_srtl_ylen1xk2vx2lo1xvx2lo1xk2vx2lo1xvx2lo1xhi1xvx2vx2hi1xk2k2hi1xvx2vx2hi1x_627 into H_srtl_xlen1xk2vx2lo1xvx2lo1xk2vx2lo1xvx2lo1xhi1xvx2vx2hi1xk2k2hi1xvx2vx2hi1x_627.
 ssl_write (x .+ 1).
 ssl_write_post (x .+ 1).
 ssl_write r.
 ssl_write_post r.
 ssl_emp;
 exists ((if ((if (hi1x) <= (vx2) then vx2 else hi1x)) <= (k2) then k2 else (if (hi1x) <= (vx2) then vx2 else hi1x))), ((if (k2) <= ((if (vx2) <= (lo1x) then vx2 else lo1x)) then k2 else (if (vx2) <= (lo1x) then vx2 else lo1x))), (((1) + (len1x)) + (1)), (x);
-exists (x :-> vx2 \+ x .+ 1 :-> y12 \+ h_srtl_y12len1xk2lo1xk2lo1xhi1xk2k2hi1x_5221);
+exists (x :-> vx2 \+ x .+ 1 :-> y12 \+ h_srtl_y12len1xk2lo1xk2lo1xhi1xk2k2hi1x_6271);
 sslauto.
-unfold_constructor 2;
-exists ((len1x) + (1)), (vx2), ((if (hi1x) <= (k2) then k2 else hi1x)), ((if (k2) <= (lo1x) then k2 else lo1x)), (y12), (h_srtl_y12len1xk2lo1xk2lo1xhi1xk2k2hi1x_5221);
+ssl_close 2;
+exists ((len1x) + (1)), (vx2), ((if (hi1x) <= (k2) then k2 else hi1x)), ((if (k2) <= (lo1x) then k2 else lo1x)), (y12), (h_srtl_y12len1xk2lo1xk2lo1xhi1xk2k2hi1x_6271);
 sslauto.
 ssl_frame_unfold.
 ssl_read (x .+ 1).
 try rename nxtx into nxtx2.
-try rename h_srtl_nxtxlen1xlo1xhi1x_520x into h_srtl_nxtx2len1xlo1xhi1x_520x.
-try rename H_srtl_nxtxlen1xlo1xhi1x_520x into H_srtl_nxtx2len1xlo1xhi1x_520x.
-try rename h_srtl_nxtylen1ylo11yhi11y_520y into h_srtl_nxtylen1ylo11yhi11nxtyvnxtyvnxtyhi11nxty_520y.
-try rename H_srtl_nxtylen1ylo11yhi11y_520y into H_srtl_nxtylen1ylo11yhi11nxtyvnxtyvnxtyhi11nxty_520y.
-try rename h_srtl_nxtylen1ylo11yhi11nxtyvnxtyvnxtyhi11nxty_520y into h_srtl_nxtylen1nxtylo11yhi11nxtyvnxtyvnxtyhi11nxty_520y.
-try rename H_srtl_nxtylen1ylo11yhi11nxtyvnxtyvnxtyhi11nxty_520y into H_srtl_nxtylen1nxtylo11yhi11nxtyvnxtyvnxtyhi11nxty_520y.
-try rename h_srtl_nxtylen1nxtylo11yhi11nxtyvnxtyvnxtyhi11nxty_520y into h_srtl_nxtylen1nxtyvnxtylo11nxtyvnxtylo11nxtyhi11nxtyvnxtyvnxtyhi11nxty_520y.
-try rename H_srtl_nxtylen1nxtylo11yhi11nxtyvnxtyvnxtyhi11nxty_520y into H_srtl_nxtylen1nxtyvnxtylo11nxtyvnxtylo11nxtyhi11nxtyvnxtyvnxtyhi11nxty_520y.
-try rename h_srtl_nxtnxtylen1nxtylo11nxtyhi11nxty_520nxty into h_srtl_nxtx2len1xlo1xhi1x_520x.
-try rename H_srtl_nxtnxtylen1nxtylo11nxtyhi11nxty_520nxty into H_srtl_nxtx2len1xlo1xhi1x_520x.
-try rename h_srtl_nxtylen1nxtyvnxtylo11nxtyvnxtylo11nxtyhi11nxtyvnxtyvnxtyhi11nxty_520y into h_srtl_nxtylen1nxtyvnxtylo11nxtyvnxtylo11nxtyhi1xvnxtyvnxtyhi1x_520y.
-try rename H_srtl_nxtylen1nxtyvnxtylo11nxtyvnxtylo11nxtyhi11nxtyvnxtyvnxtyhi11nxty_520y into H_srtl_nxtylen1nxtyvnxtylo11nxtyvnxtylo11nxtyhi1xvnxtyvnxtyhi1x_520y.
-try rename h_srtl_nxtylen1nxtyvnxtylo11nxtyvnxtylo11nxtyhi1xvnxtyvnxtyhi1x_520y into h_srtl_nxtylen1xvnxtylo11nxtyvnxtylo11nxtyhi1xvnxtyvnxtyhi1x_520y.
-try rename H_srtl_nxtylen1nxtyvnxtylo11nxtyvnxtylo11nxtyhi1xvnxtyvnxtyhi1x_520y into H_srtl_nxtylen1xvnxtylo11nxtyvnxtylo11nxtyhi1xvnxtyvnxtyhi1x_520y.
-try rename h_srtl_nxtylen1xvnxtylo11nxtyvnxtylo11nxtyhi1xvnxtyvnxtyhi1x_520y into h_srtl_nxtylen1xvnxtylo1xvnxtylo1xhi1xvnxtyvnxtyhi1x_520y.
-try rename H_srtl_nxtylen1xvnxtylo11nxtyvnxtylo11nxtyhi1xvnxtyvnxtyhi1x_520y into H_srtl_nxtylen1xvnxtylo1xvnxtylo1xhi1xvnxtyvnxtyhi1x_520y.
-try rename h_srtl_ylen1xk2vx2lo1xvx2lo1xk2vx2lo1xvx2lo1xhi1xvx2vx2hi1xk2k2hi1xvx2vx2hi1x_522 into h_srtl_xlen1xk2vx2lo1xvx2lo1xk2vx2lo1xvx2lo1xhi1xvx2vx2hi1xk2k2hi1xvx2vx2hi1x_522.
-try rename H_srtl_ylen1xk2vx2lo1xvx2lo1xk2vx2lo1xvx2lo1xhi1xvx2vx2hi1xk2k2hi1xvx2vx2hi1x_522 into H_srtl_xlen1xk2vx2lo1xvx2lo1xk2vx2lo1xvx2lo1xhi1xvx2vx2hi1xk2k2hi1xvx2vx2hi1x_522.
+try rename h_srtl_nxtxlen1xlo1xhi1x_625x into h_srtl_nxtx2len1xlo1xhi1x_625x.
+try rename H_srtl_nxtxlen1xlo1xhi1x_625x into H_srtl_nxtx2len1xlo1xhi1x_625x.
+try rename h_srtl_nxtylen1ylo11yhi11y_625y into h_srtl_nxtylen1ylo11yhi11nxtyvnxtyvnxtyhi11nxty_625y.
+try rename H_srtl_nxtylen1ylo11yhi11y_625y into H_srtl_nxtylen1ylo11yhi11nxtyvnxtyvnxtyhi11nxty_625y.
+try rename h_srtl_nxtylen1ylo11yhi11nxtyvnxtyvnxtyhi11nxty_625y into h_srtl_nxtylen1nxtylo11yhi11nxtyvnxtyvnxtyhi11nxty_625y.
+try rename H_srtl_nxtylen1ylo11yhi11nxtyvnxtyvnxtyhi11nxty_625y into H_srtl_nxtylen1nxtylo11yhi11nxtyvnxtyvnxtyhi11nxty_625y.
+try rename h_srtl_nxtylen1nxtylo11yhi11nxtyvnxtyvnxtyhi11nxty_625y into h_srtl_nxtylen1nxtyvnxtylo11nxtyvnxtylo11nxtyhi11nxtyvnxtyvnxtyhi11nxty_625y.
+try rename H_srtl_nxtylen1nxtylo11yhi11nxtyvnxtyvnxtyhi11nxty_625y into H_srtl_nxtylen1nxtyvnxtylo11nxtyvnxtylo11nxtyhi11nxtyvnxtyvnxtyhi11nxty_625y.
+try rename h_srtl_nxtnxtylen1nxtylo11nxtyhi11nxty_625nxty into h_srtl_nxtx2len1xlo1xhi1x_625x.
+try rename H_srtl_nxtnxtylen1nxtylo11nxtyhi11nxty_625nxty into H_srtl_nxtx2len1xlo1xhi1x_625x.
+try rename h_srtl_nxtylen1nxtyvnxtylo11nxtyvnxtylo11nxtyhi11nxtyvnxtyvnxtyhi11nxty_625y into h_srtl_nxtylen1nxtyvnxtylo11nxtyvnxtylo11nxtyhi1xvnxtyvnxtyhi1x_625y.
+try rename H_srtl_nxtylen1nxtyvnxtylo11nxtyvnxtylo11nxtyhi11nxtyvnxtyvnxtyhi11nxty_625y into H_srtl_nxtylen1nxtyvnxtylo11nxtyvnxtylo11nxtyhi1xvnxtyvnxtyhi1x_625y.
+try rename h_srtl_nxtylen1nxtyvnxtylo11nxtyvnxtylo11nxtyhi1xvnxtyvnxtyhi1x_625y into h_srtl_nxtylen1xvnxtylo11nxtyvnxtylo11nxtyhi1xvnxtyvnxtyhi1x_625y.
+try rename H_srtl_nxtylen1nxtyvnxtylo11nxtyvnxtylo11nxtyhi1xvnxtyvnxtyhi1x_625y into H_srtl_nxtylen1xvnxtylo11nxtyvnxtylo11nxtyhi1xvnxtyvnxtyhi1x_625y.
+try rename h_srtl_nxtylen1xvnxtylo11nxtyvnxtylo11nxtyhi1xvnxtyvnxtyhi1x_625y into h_srtl_nxtylen1xvnxtylo1xvnxtylo1xhi1xvnxtyvnxtyhi1x_625y.
+try rename H_srtl_nxtylen1xvnxtylo11nxtyvnxtylo11nxtyhi1xvnxtyvnxtyhi1x_625y into H_srtl_nxtylen1xvnxtylo1xvnxtylo1xhi1xvnxtyvnxtyhi1x_625y.
+try rename h_srtl_ylen1xk2vx2lo1xvx2lo1xk2vx2lo1xvx2lo1xhi1xvx2vx2hi1xk2k2hi1xvx2vx2hi1x_627 into h_srtl_xlen1xk2vx2lo1xvx2lo1xk2vx2lo1xvx2lo1xhi1xvx2vx2hi1xk2k2hi1xvx2vx2hi1x_627.
+try rename H_srtl_ylen1xk2vx2lo1xvx2lo1xk2vx2lo1xvx2lo1xhi1xvx2vx2hi1xk2k2hi1xvx2vx2hi1x_627 into H_srtl_xlen1xk2vx2lo1xvx2lo1xk2vx2lo1xvx2lo1xhi1xvx2vx2hi1xk2k2hi1xvx2vx2hi1x_627.
 ssl_alloc nxty2.
 try rename nxty into nxty2.
-try rename h_srtl_nxtylen1xvnxtylo1xvnxtylo1xhi1xvnxtyvnxtyhi1x_520y into h_srtl_nxty2len1xvnxtylo1xvnxtylo1xhi1xvnxtyvnxtyhi1x_520y.
-try rename H_srtl_nxtylen1xvnxtylo1xvnxtylo1xhi1xvnxtyvnxtyhi1x_520y into H_srtl_nxty2len1xvnxtylo1xvnxtylo1xhi1xvnxtyvnxtyhi1x_520y.
+try rename h_srtl_nxtylen1xvnxtylo1xvnxtylo1xhi1xvnxtyvnxtyhi1x_625y into h_srtl_nxty2len1xvnxtylo1xvnxtylo1xhi1xvnxtyvnxtyhi1x_625y.
+try rename H_srtl_nxtylen1xvnxtylo1xvnxtylo1xhi1xvnxtyvnxtyhi1x_625y into H_srtl_nxty2len1xvnxtylo1xvnxtylo1xhi1xvnxtyvnxtyhi1x_625y.
 ssl_write (x .+ 1).
 ssl_write_post (x .+ 1).
 ssl_write r.
 ssl_write_post r.
 ssl_write (nxty2 .+ 1).
 ssl_write_post (nxty2 .+ 1).
-try rename h_srtl_nxty2len1xvnxtylo1xvnxtylo1xhi1xvnxtyvnxtyhi1x_520y into h_srtl_nxty2len1xvx2lo1xvx2lo1xhi1xvx2vx2hi1x_520y.
-try rename H_srtl_nxty2len1xvnxtylo1xvnxtylo1xhi1xvnxtyvnxtyhi1x_520y into H_srtl_nxty2len1xvx2lo1xvx2lo1xhi1xvx2vx2hi1x_520y.
+try rename h_srtl_nxty2len1xvnxtylo1xvnxtylo1xhi1xvnxtyvnxtyhi1x_625y into h_srtl_nxty2len1xvx2lo1xvx2lo1xhi1xvx2vx2hi1x_625y.
+try rename H_srtl_nxty2len1xvnxtylo1xvnxtylo1xhi1xvnxtyvnxtyhi1x_625y into H_srtl_nxty2len1xvx2lo1xvx2lo1xhi1xvx2vx2hi1x_625y.
 ssl_write x.
 ssl_write_post x.
 ssl_write nxty2.
 ssl_write_post nxty2.
 ssl_emp;
 exists ((if ((if (hi1x) <= (vx2) then vx2 else hi1x)) <= (k2) then k2 else (if (hi1x) <= (vx2) then vx2 else hi1x))), ((if (k2) <= ((if (vx2) <= (lo1x) then vx2 else lo1x)) then k2 else (if (vx2) <= (lo1x) then vx2 else lo1x))), (((1) + (len1x)) + (1)), (x);
-exists (x :-> k2 \+ x .+ 1 :-> nxty2 \+ nxty2 :-> vx2 \+ nxty2 .+ 1 :-> nxtx2 \+ h_srtl_nxtx2len1xlo1xhi1x_520x);
+exists (x :-> k2 \+ x .+ 1 :-> nxty2 \+ nxty2 :-> vx2 \+ nxty2 .+ 1 :-> nxtx2 \+ h_srtl_nxtx2len1xlo1xhi1x_625x);
 sslauto.
-unfold_constructor 2;
-exists ((1) + (len1x)), (k2), ((if (hi1x) <= (vx2) then vx2 else hi1x)), ((if (vx2) <= (lo1x) then vx2 else lo1x)), (nxty2), (nxty2 :-> vx2 \+ nxty2 .+ 1 :-> nxtx2 \+ h_srtl_nxtx2len1xlo1xhi1x_520x);
+ssl_close 2;
+exists ((1) + (len1x)), (k2), ((if (hi1x) <= (vx2) then vx2 else hi1x)), ((if (vx2) <= (lo1x) then vx2 else lo1x)), (nxty2), (nxty2 :-> vx2 \+ nxty2 .+ 1 :-> nxtx2 \+ h_srtl_nxtx2len1xlo1xhi1x_625x);
 sslauto.
-unfold_constructor 2;
-exists (len1x), (vx2), (hi1x), (lo1x), (nxtx2), (h_srtl_nxtx2len1xlo1xhi1x_520x);
+ssl_close 2;
+exists (len1x), (vx2), (hi1x), (lo1x), (nxtx2), (h_srtl_nxtx2len1xlo1xhi1x_625x);
 sslauto.
 ssl_frame_unfold.
 Qed.
