examples/srtl_prepend.v
@@ -12,21 +12,21 @@ Inductive sll (x : ptr) (len : nat) (lo : nat) (hi : nat) (h : heap) : Prop :=
   (hi) == (0) /\ (len) == (0) /\ (lo) == (7) /\ h = empty
 | sll_2 of ~~ ((x) == (null)) of
   exists (len1 : nat) (v : nat) (hi1 : nat) (lo1 : nat) (nxt : ptr),
-  exists h_sll_nxtlen1lo1hi1_523,
-  (0) <= (len1) /\ (0) <= (v) /\ (hi) == ((if (hi1) <= (v) then v else hi1)) /\ (len) == ((1) + (len1)) /\ (lo) == ((if (v) <= (lo1) then v else lo1)) /\ (v) <= (7) /\ h = x :-> v \+ x .+ 1 :-> nxt \+ h_sll_nxtlen1lo1hi1_523 /\ sll nxt len1 lo1 hi1 h_sll_nxtlen1lo1hi1_523.
+  exists h_sll_nxtlen1lo1hi1_628,
+  (0) <= (len1) /\ (0) <= (v) /\ (hi) == ((if (hi1) <= (v) then v else hi1)) /\ (len) == ((1) + (len1)) /\ (lo) == ((if (v) <= (lo1) then v else lo1)) /\ (v) <= (7) /\ h = x :-> v \+ x .+ 1 :-> nxt \+ h_sll_nxtlen1lo1hi1_628 /\ sll nxt len1 lo1 hi1 h_sll_nxtlen1lo1hi1_628.
 
 Inductive srtl (x : ptr) (len : nat) (lo : nat) (hi : nat) (h : heap) : Prop :=
 | srtl_1 of (x) == (null) of
   (hi) == (0) /\ (len) == (0) /\ (lo) == (7) /\ h = empty
 | srtl_2 of ~~ ((x) == (null)) of
   exists (len1 : nat) (v : nat) (hi1 : nat) (lo1 : nat) (nxt : ptr),
-  exists h_srtl_nxtlen1lo1hi1_524,
-  (0) <= (len1) /\ (0) <= (v) /\ (hi) == ((if (hi1) <= (v) then v else hi1)) /\ (len) == ((1) + (len1)) /\ (lo) == ((if (v) <= (lo1) then v else lo1)) /\ (v) <= (7) /\ (v) <= (lo1) /\ h = x :-> v \+ x .+ 1 :-> nxt \+ h_srtl_nxtlen1lo1hi1_524 /\ srtl nxt len1 lo1 hi1 h_srtl_nxtlen1lo1hi1_524.
+  exists h_srtl_nxtlen1lo1hi1_629,
+  (0) <= (len1) /\ (0) <= (v) /\ (hi) == ((if (hi1) <= (v) then v else hi1)) /\ (len) == ((1) + (len1)) /\ (lo) == ((if (v) <= (lo1) then v else lo1)) /\ (v) <= (7) /\ (v) <= (lo1) /\ h = x :-> v \+ x .+ 1 :-> nxt \+ h_srtl_nxtlen1lo1hi1_629 /\ srtl nxt len1 lo1 hi1 h_srtl_nxtlen1lo1hi1_629.
 
-Lemma pure24 n : (0) <= (n) -> ((n) + (1)) == ((1) + (n)). Admitted.
-Hint Resolve pure24: ssl_pure.
-Lemma pure25 k lo : (k) <= (7) -> (k) <= (lo) -> (0) <= (k) -> (k) == ((if (k) <= (lo) then k else lo)). Admitted.
-Hint Resolve pure25: ssl_pure.
+Lemma pure151 n : (0) <= (n) -> ((n) + (1)) = ((1) + (n)). Admitted.
+Hint Resolve pure151: ssl_pure.
+Lemma pure152 k lo : (0) <= (k) -> (k) <= (7) -> (k) <= (lo) -> (k) = ((if (k) <= (lo) then k else lo)). Admitted.
+Hint Resolve pure152: ssl_pure.
 
 Definition srtl_prepend_type :=
   forall (vprogs : ptr * nat * ptr),
@@ -35,14 +35,14 @@ Definition srtl_prepend_type :=
     fun h =>
       let: (x, k, r) := vprogs in
       let: (n, lo, hi, a) := vghosts in
-      exists h_srtl_xnlohi_525,
-      (0) <= (k) /\ (0) <= (n) /\ (k) <= (7) /\ (k) <= (lo) /\ h = r :-> a \+ h_srtl_xnlohi_525 /\ srtl x n lo hi h_srtl_xnlohi_525,
+      exists h_srtl_xnlohi_630,
+      (0) <= (k) /\ (0) <= (n) /\ (k) <= (7) /\ (k) <= (lo) /\ h = r :-> a \+ h_srtl_xnlohi_630 /\ srtl x n lo hi h_srtl_xnlohi_630,
     [vfun (_: unit) h =>
       let: (x, k, r) := vprogs in
       let: (n, lo, hi, a) := vghosts in
       exists n1 y hi1,
-      exists h_srtl_yn1khi1_526,
-      (n1) == ((n) + (1)) /\ h = r :-> y \+ h_srtl_yn1khi1_526 /\ srtl y n1 k hi1 h_srtl_yn1khi1_526
+      exists h_srtl_yn1khi1_631,
+      (n1) == ((n) + (1)) /\ h = r :-> y \+ h_srtl_yn1khi1_631 /\ srtl y n1 k hi1 h_srtl_yn1khi1_631
     ]).
 
 Program Definition srtl_prepend : srtl_prepend_type :=
@@ -60,40 +60,40 @@ Obligation Tactic := intro; move=>[[x k] r]; ssl_program_simpl.
 Next Obligation.
 ssl_ghostelim_pre.
 move=>[[[n lo] hi] a].
-ex_elim h_srtl_xnlohi_525.
+ex_elim h_srtl_xnlohi_630.
 move=>[phi_self0] [phi_self1] [phi_self2] [phi_self3].
 move=>[sigma_self].
 subst h_self.
-move=>H_srtl_xnlohi_525.
+move=>H_srtl_xnlohi_630.
 ssl_ghostelim_post.
-try rename h_srtl_yn1khi1_526 into h_srtl_ynkhi1_526.
-try rename H_srtl_yn1khi1_526 into H_srtl_ynkhi1_526.
+try rename h_srtl_yn1khi1_631 into h_srtl_ynkhi1_631.
+try rename H_srtl_yn1khi1_631 into H_srtl_ynkhi1_631.
 ssl_read r.
 try rename a into a2.
-try rename h_srtl_ynkhi1_526 into h_srtl_ynkhi11yvyvyhi11y_526.
-try rename H_srtl_ynkhi1_526 into H_srtl_ynkhi11yvyvyhi11y_526.
-try rename h_srtl_nxtylen1ylo1yhi11y_524y into h_srtl_xnlohi_525.
-try rename H_srtl_nxtylen1ylo1yhi11y_524y into H_srtl_xnlohi_525.
-try rename h_srtl_ynkhi11yvyvyhi11y_526 into h_srtl_ynkhivyvyhi_526.
-try rename H_srtl_ynkhi11yvyvyhi11y_526 into H_srtl_ynkhivyvyhi_526.
+try rename h_srtl_ynkhi1_631 into h_srtl_ynkhi11yvyvyhi11y_631.
+try rename H_srtl_ynkhi1_631 into H_srtl_ynkhi11yvyvyhi11y_631.
+try rename h_srtl_nxtylen1ylo1yhi11y_629y into h_srtl_xnlohi_630.
+try rename H_srtl_nxtylen1ylo1yhi11y_629y into H_srtl_xnlohi_630.
+try rename h_srtl_ynkhi11yvyvyhi11y_631 into h_srtl_ynkhivyvyhi_631.
+try rename H_srtl_ynkhi11yvyvyhi11y_631 into H_srtl_ynkhivyvyhi_631.
 ssl_alloc y2.
 try rename y into y2.
-try rename h_srtl_ynkhivyvyhi_526 into h_srtl_y2nkhivyvyhi_526.
-try rename H_srtl_ynkhivyvyhi_526 into H_srtl_y2nkhivyvyhi_526.
+try rename h_srtl_ynkhivyvyhi_631 into h_srtl_y2nkhivyvyhi_631.
+try rename H_srtl_ynkhivyvyhi_631 into H_srtl_y2nkhivyvyhi_631.
 ssl_write r.
 ssl_write_post r.
 ssl_write (y2 .+ 1).
 ssl_write_post (y2 .+ 1).
-try rename h_srtl_y2nkhivyvyhi_526 into h_srtl_y2nkhikkhi_526.
-try rename H_srtl_y2nkhivyvyhi_526 into H_srtl_y2nkhikkhi_526.
+try rename h_srtl_y2nkhivyvyhi_631 into h_srtl_y2nkhikkhi_631.
+try rename H_srtl_y2nkhivyvyhi_631 into H_srtl_y2nkhikkhi_631.
 ssl_write y2.
 ssl_write_post y2.
 ssl_emp;
 exists ((n) + (1)), (y2), ((if (hi) <= (k) then k else hi));
-exists (y2 :-> k \+ y2 .+ 1 :-> x \+ h_srtl_xnlohi_525);
+exists (y2 :-> k \+ y2 .+ 1 :-> x \+ h_srtl_xnlohi_630);
 sslauto.
-unfold_constructor 2;
-exists (n), (k), (hi), (lo), (x), (h_srtl_xnlohi_525);
+ssl_close 2;
+exists (n), (k), (hi), (lo), (x), (h_srtl_xnlohi_630);
 sslauto.
 ssl_frame_unfold.
 Qed.
