examples/bst_right_rotate.v
@@ -12,17 +12,17 @@ Inductive bst (x : ptr) (sz : nat) (lo : nat) (hi : nat) (h : heap) : Prop :=
   (hi) == (0) /\ (lo) == (7) /\ (sz) == (0) /\ h = empty
 | bst_2 of ~~ ((x) == (null)) of
   exists (sz1 : nat) (sz2 : nat) (v : nat) (hi2 : nat) (hi1 : nat) (lo1 : nat) (lo2 : nat) (l : ptr) (r : ptr),
-  exists h_bst_lsz1lo1hi1_525 h_bst_rsz2lo2hi2_526,
-  (0) <= (sz1) /\ (0) <= (sz2) /\ (0) <= (v) /\ (hi) == ((if (hi2) <= (v) then v else hi2)) /\ (hi1) <= (v) /\ (lo) == ((if (v) <= (lo1) then v else lo1)) /\ (sz) == (((1) + (sz1)) + (sz2)) /\ (v) <= (7) /\ (v) <= (lo2) /\ h = x :-> v \+ x .+ 1 :-> l \+ x .+ 2 :-> r \+ h_bst_lsz1lo1hi1_525 \+ h_bst_rsz2lo2hi2_526 /\ bst l sz1 lo1 hi1 h_bst_lsz1lo1hi1_525 /\ bst r sz2 lo2 hi2 h_bst_rsz2lo2hi2_526.
+  exists h_bst_lsz1lo1hi1_614 h_bst_rsz2lo2hi2_615,
+  (0) <= (sz1) /\ (0) <= (sz2) /\ (0) <= (v) /\ (hi) == ((if (hi2) <= (v) then v else hi2)) /\ (hi1) <= (v) /\ (lo) == ((if (v) <= (lo1) then v else lo1)) /\ (sz) == (((1) + (sz1)) + (sz2)) /\ (v) <= (7) /\ (v) <= (lo2) /\ h = x :-> v \+ x .+ 1 :-> l \+ x .+ 2 :-> r \+ h_bst_lsz1lo1hi1_614 \+ h_bst_rsz2lo2hi2_615 /\ bst l sz1 lo1 hi1 h_bst_lsz1lo1hi1_614 /\ bst r sz2 lo2 hi2 h_bst_rsz2lo2hi2_615.
 
-Lemma pure39 sz2l2 sz2 sz1l2 : (0) <= (sz2l2) -> (0) <= (((1) + (sz1l2)) + (sz2l2)) -> (0) <= (sz2) -> (0) <= (sz1l2) -> (0) <= (((1) + (sz2l2)) + (sz2)). Admitted.
-Hint Resolve pure39: ssl_pure.
-Lemma pure40 sz1l2 sz2l2 sz2 : (0) <= (sz2l2) -> (0) <= (((1) + (sz1l2)) + (sz2l2)) -> (0) <= (sz2) -> (0) <= (sz1l2) -> ((sz1l2) + (((1) + (sz2l2)) + (sz2))) == ((((1) + (sz1l2)) + (sz2l2)) + (sz2)). Admitted.
-Hint Resolve pure40: ssl_pure.
-Lemma pure41 lo2l2 v2 vl22 hi2l2 lo2 hi1l2 : (v2) <= (lo2) -> (v2) <= (7) -> (hi1l2) <= (vl22) -> ((if (hi2l2) <= (vl22) then vl22 else hi2l2)) <= (v2) -> (0) <= (v2) -> (vl22) <= (lo2l2) -> (vl22) <= (7) -> (0) <= (vl22) -> (hi2l2) <= (v2). Admitted.
-Hint Resolve pure41: ssl_pure.
-Lemma pure42 lo2l2 v2 vl22 hi2l2 lo2 hi1l2 : (v2) <= (lo2) -> (v2) <= (7) -> (hi1l2) <= (vl22) -> ((if (hi2l2) <= (vl22) then vl22 else hi2l2)) <= (v2) -> (0) <= (v2) -> (vl22) <= (lo2l2) -> (vl22) <= (7) -> (0) <= (vl22) -> (vl22) <= ((if (v2) <= (lo2l2) then v2 else lo2l2)). Admitted.
-Hint Resolve pure42: ssl_pure.
+Lemma pure124 sz1l2 sz2l2 sz2 : (0) <= (sz2l2) -> (0) <= (((1) + (sz1l2)) + (sz2l2)) -> (0) <= (sz2) -> (0) <= (sz1l2) -> ((sz1l2) + (((1) + (sz2l2)) + (sz2))) = ((((1) + (sz1l2)) + (sz2l2)) + (sz2)). Admitted.
+Hint Resolve pure124: ssl_pure.
+Lemma pure125 sz2l2 sz2 sz1l2 : (0) <= (sz2l2) -> (0) <= (((1) + (sz1l2)) + (sz2l2)) -> (0) <= (sz2) -> (0) <= (sz1l2) -> (0) <= (((1) + (sz2l2)) + (sz2)). Admitted.
+Hint Resolve pure125: ssl_pure.
+Lemma pure126 lo2l2 v2 vl22 hi2l2 lo2 hi1l2 : (v2) <= (lo2) -> (v2) <= (7) -> (hi1l2) <= (vl22) -> ((if (hi2l2) <= (vl22) then vl22 else hi2l2)) <= (v2) -> (0) <= (v2) -> (vl22) <= (lo2l2) -> (vl22) <= (7) -> (0) <= (vl22) -> (vl22) <= ((if (v2) <= (lo2l2) then v2 else lo2l2)). Admitted.
+Hint Resolve pure126: ssl_pure.
+Lemma pure127 lo2l2 v2 vl22 hi2l2 lo2 hi1l2 : (v2) <= (lo2) -> (v2) <= (7) -> (hi1l2) <= (vl22) -> ((if (hi2l2) <= (vl22) then vl22 else hi2l2)) <= (v2) -> (0) <= (v2) -> (vl22) <= (lo2l2) -> (vl22) <= (7) -> (0) <= (vl22) -> (hi2l2) <= (v2). Admitted.
+Hint Resolve pure127: ssl_pure.
 
 Definition bst_right_rotate_type :=
   forall (vprogs : ptr * ptr),
@@ -37,8 +37,8 @@ Definition bst_right_rotate_type :=
       let: (x, retv) := vprogs in
       let: (sz1, sz2, v, hi1, l, lo2, lo1, r, hi2, unused) := vghosts in
       exists sz3 sz4 v3 hi3 lo4 l3 lo3 hi4 y,
-      exists h_bst_l3sz3lo3hi3_527 h_bst_xsz4lo4hi4_528,
-      (0) <= (sz3) /\ (0) <= (sz4) /\ (0) <= (v3) /\ (hi3) <= (v3) /\ ((sz3) + (sz4)) == ((sz1) + (sz2)) /\ (v3) <= (7) /\ (v3) <= (lo4) /\ h = retv :-> y \+ y :-> v3 \+ y .+ 1 :-> l3 \+ y .+ 2 :-> x \+ h_bst_l3sz3lo3hi3_527 \+ h_bst_xsz4lo4hi4_528 /\ bst l3 sz3 lo3 hi3 h_bst_l3sz3lo3hi3_527 /\ bst x sz4 lo4 hi4 h_bst_xsz4lo4hi4_528
+      exists h_bst_l3sz3lo3hi3_616 h_bst_xsz4lo4hi4_617,
+      (0) <= (sz3) /\ (0) <= (sz4) /\ (0) <= (v3) /\ (hi3) <= (v3) /\ ((sz3) + (sz4)) == ((sz1) + (sz2)) /\ (v3) <= (7) /\ (v3) <= (lo4) /\ h = retv :-> y \+ y :-> v3 \+ y .+ 1 :-> l3 \+ y .+ 2 :-> x \+ h_bst_l3sz3lo3hi3_616 \+ h_bst_xsz4lo4hi4_617 /\ bst l3 sz3 lo3 hi3 h_bst_l3sz3lo3hi3_616 /\ bst x sz4 lo4 hi4 h_bst_xsz4lo4hi4_617
     ]).
 
 Program Definition bst_right_rotate : bst_right_rotate_type :=
@@ -90,11 +90,11 @@ subst h_bst_l2sz1lo1hi1_a.
 ssl_inconsistency.
 ex_elim sz1l2 sz2l2 vl2 hi2l2 hi1l2.
 ex_elim lo1l2 lo2l2 ll2 rl2.
-ex_elim h_bst_ll2sz1l2lo1l2hi1l2_525l2 h_bst_rl2sz2l2lo2l2hi2l2_526l2.
+ex_elim h_bst_ll2sz1l2lo1l2hi1l2_614l2 h_bst_rl2sz2l2lo2l2hi2l2_615l2.
 move=>[phi_bst_l2sz1lo1hi1_a0] [phi_bst_l2sz1lo1hi1_a1] [phi_bst_l2sz1lo1hi1_a2] [phi_bst_l2sz1lo1hi1_a3] [phi_bst_l2sz1lo1hi1_a4] [phi_bst_l2sz1lo1hi1_a5] [phi_bst_l2sz1lo1hi1_a6] [phi_bst_l2sz1lo1hi1_a7] [phi_bst_l2sz1lo1hi1_a8].
 move=>[sigma_bst_l2sz1lo1hi1_a].
 subst h_bst_l2sz1lo1hi1_a.
-move=>[H_bst_ll2sz1l2lo1l2hi1l2_525l2 H_bst_rl2sz2l2lo2l2hi2l2_526l2].
+move=>[H_bst_ll2sz1l2lo1l2hi1l2_614l2 H_bst_rl2sz2l2lo2l2hi2l2_615l2].
 try rename h_bst_l2sz1lo1hi1_a into h_bst_l2sz1lo1hi2l2vl2vl2hi2l2_a.
 try rename H_bst_l2sz1lo1hi1_a into H_bst_l2sz1lo1hi2l2vl2vl2hi2l2_a.
 try rename h_bst_l2sz1lo1hi2l2vl2vl2hi2l2_a into h_bst_l2sz1vl2lo1l2vl2lo1l2hi2l2vl2vl2hi2l2_a.
@@ -107,48 +107,48 @@ try rename h_bst_l2sz1l2sz2l2vl2lo1l2vl2lo1l2hi2l2vl2vl2hi2l2_a into h_bst_l2sz1
 try rename H_bst_l2sz1l2sz2l2vl2lo1l2vl2lo1l2hi2l2vl2vl2hi2l2_a into H_bst_l2sz1l2sz2l2vl22lo1l2vl22lo1l2hi2l2vl22vl22hi2l2_a.
 ssl_read (l2 .+ 1).
 try rename ll2 into ll22.
-try rename h_bst_ll2sz1l2lo1l2hi1l2_525l2 into h_bst_ll22sz1l2lo1l2hi1l2_525l2.
-try rename H_bst_ll2sz1l2lo1l2hi1l2_525l2 into H_bst_ll22sz1l2lo1l2hi1l2_525l2.
+try rename h_bst_ll2sz1l2lo1l2hi1l2_614l2 into h_bst_ll22sz1l2lo1l2hi1l2_614l2.
+try rename H_bst_ll2sz1l2lo1l2hi1l2_614l2 into H_bst_ll22sz1l2lo1l2hi1l2_614l2.
 ssl_read (l2 .+ 2).
 try rename rl2 into rl22.
-try rename h_bst_rl2sz2l2lo2l2hi2l2_526l2 into h_bst_rl22sz2l2lo2l2hi2l2_526l2.
-try rename H_bst_rl2sz2l2lo2l2hi2l2_526l2 into H_bst_rl22sz2l2lo2l2hi2l2_526l2.
-try rename h_bst_xsz4lo4hi4_528 into h_bst_xsz4lo4hi21xv1xv1xhi21x_528.
-try rename H_bst_xsz4lo4hi4_528 into H_bst_xsz4lo4hi21xv1xv1xhi21x_528.
-try rename h_bst_xsz4lo4hi21xv1xv1xhi21x_528 into h_bst_xsz4v1xlo11xv1xlo11xhi21xv1xv1xhi21x_528.
-try rename H_bst_xsz4lo4hi21xv1xv1xhi21x_528 into H_bst_xsz4v1xlo11xv1xlo11xhi21xv1xv1xhi21x_528.
-try rename h_bst_xsz4v1xlo11xv1xlo11xhi21xv1xv1xhi21x_528 into h_bst_xsz11xsz21xv1xlo11xv1xlo11xhi21xv1xv1xhi21x_528.
-try rename H_bst_xsz4v1xlo11xv1xlo11xhi21xv1xv1xhi21x_528 into H_bst_xsz11xsz21xv1xlo11xv1xlo11xhi21xv1xv1xhi21x_528.
-try rename h_bst_l3sz3lo3hi3_527 into h_bst_ll22sz1l2lo1l2hi1l2_525l2.
-try rename H_bst_l3sz3lo3hi3_527 into H_bst_ll22sz1l2lo1l2hi1l2_525l2.
-try rename h_bst_l1xsz11xlo11xhi11x_525x into h_bst_rl22sz2l2lo2l2hi2l2_526l2.
-try rename H_bst_l1xsz11xlo11xhi11x_525x into H_bst_rl22sz2l2lo2l2hi2l2_526l2.
-try rename h_bst_xsz11xsz21xv1xlo11xv1xlo11xhi21xv1xv1xhi21x_528 into h_bst_xsz11xsz21xv1xlo2l2v1xlo2l2hi21xv1xv1xhi21x_528.
-try rename H_bst_xsz11xsz21xv1xlo11xv1xlo11xhi21xv1xv1xhi21x_528 into H_bst_xsz11xsz21xv1xlo2l2v1xlo2l2hi21xv1xv1xhi21x_528.
-try rename h_bst_xsz11xsz21xv1xlo2l2v1xlo2l2hi21xv1xv1xhi21x_528 into h_bst_xsz2l2sz21xv1xlo2l2v1xlo2l2hi21xv1xv1xhi21x_528.
-try rename H_bst_xsz11xsz21xv1xlo2l2v1xlo2l2hi21xv1xv1xhi21x_528 into H_bst_xsz2l2sz21xv1xlo2l2v1xlo2l2hi21xv1xv1xhi21x_528.
-try rename h_bst_r1xsz21xlo21xhi21x_526x into h_bst_r2sz2lo2hi2_b.
-try rename H_bst_r1xsz21xlo21xhi21x_526x into H_bst_r2sz2lo2hi2_b.
-try rename h_bst_xsz2l2sz21xv1xlo2l2v1xlo2l2hi21xv1xv1xhi21x_528 into h_bst_xsz2l2sz21xv1xlo2l2v1xlo2l2hi2v1xv1xhi2_528.
-try rename H_bst_xsz2l2sz21xv1xlo2l2v1xlo2l2hi21xv1xv1xhi21x_528 into H_bst_xsz2l2sz21xv1xlo2l2v1xlo2l2hi2v1xv1xhi2_528.
-try rename h_bst_xsz2l2sz21xv1xlo2l2v1xlo2l2hi2v1xv1xhi2_528 into h_bst_xsz2l2sz2v1xlo2l2v1xlo2l2hi2v1xv1xhi2_528.
-try rename H_bst_xsz2l2sz21xv1xlo2l2v1xlo2l2hi2v1xv1xhi2_528 into H_bst_xsz2l2sz2v1xlo2l2v1xlo2l2hi2v1xv1xhi2_528.
+try rename h_bst_rl2sz2l2lo2l2hi2l2_615l2 into h_bst_rl22sz2l2lo2l2hi2l2_615l2.
+try rename H_bst_rl2sz2l2lo2l2hi2l2_615l2 into H_bst_rl22sz2l2lo2l2hi2l2_615l2.
+try rename h_bst_xsz4lo4hi4_617 into h_bst_xsz4lo4hi21xv1xv1xhi21x_617.
+try rename H_bst_xsz4lo4hi4_617 into H_bst_xsz4lo4hi21xv1xv1xhi21x_617.
+try rename h_bst_xsz4lo4hi21xv1xv1xhi21x_617 into h_bst_xsz4v1xlo11xv1xlo11xhi21xv1xv1xhi21x_617.
+try rename H_bst_xsz4lo4hi21xv1xv1xhi21x_617 into H_bst_xsz4v1xlo11xv1xlo11xhi21xv1xv1xhi21x_617.
+try rename h_bst_xsz4v1xlo11xv1xlo11xhi21xv1xv1xhi21x_617 into h_bst_xsz11xsz21xv1xlo11xv1xlo11xhi21xv1xv1xhi21x_617.
+try rename H_bst_xsz4v1xlo11xv1xlo11xhi21xv1xv1xhi21x_617 into H_bst_xsz11xsz21xv1xlo11xv1xlo11xhi21xv1xv1xhi21x_617.
+try rename h_bst_l3sz3lo3hi3_616 into h_bst_ll22sz1l2lo1l2hi1l2_614l2.
+try rename H_bst_l3sz3lo3hi3_616 into H_bst_ll22sz1l2lo1l2hi1l2_614l2.
+try rename h_bst_l1xsz11xlo11xhi11x_614x into h_bst_rl22sz2l2lo2l2hi2l2_615l2.
+try rename H_bst_l1xsz11xlo11xhi11x_614x into H_bst_rl22sz2l2lo2l2hi2l2_615l2.
+try rename h_bst_xsz11xsz21xv1xlo11xv1xlo11xhi21xv1xv1xhi21x_617 into h_bst_xsz11xsz21xv1xlo2l2v1xlo2l2hi21xv1xv1xhi21x_617.
+try rename H_bst_xsz11xsz21xv1xlo11xv1xlo11xhi21xv1xv1xhi21x_617 into H_bst_xsz11xsz21xv1xlo2l2v1xlo2l2hi21xv1xv1xhi21x_617.
+try rename h_bst_xsz11xsz21xv1xlo2l2v1xlo2l2hi21xv1xv1xhi21x_617 into h_bst_xsz2l2sz21xv1xlo2l2v1xlo2l2hi21xv1xv1xhi21x_617.
+try rename H_bst_xsz11xsz21xv1xlo2l2v1xlo2l2hi21xv1xv1xhi21x_617 into H_bst_xsz2l2sz21xv1xlo2l2v1xlo2l2hi21xv1xv1xhi21x_617.
+try rename h_bst_r1xsz21xlo21xhi21x_615x into h_bst_r2sz2lo2hi2_b.
+try rename H_bst_r1xsz21xlo21xhi21x_615x into H_bst_r2sz2lo2hi2_b.
+try rename h_bst_xsz2l2sz21xv1xlo2l2v1xlo2l2hi21xv1xv1xhi21x_617 into h_bst_xsz2l2sz21xv1xlo2l2v1xlo2l2hi2v1xv1xhi2_617.
+try rename H_bst_xsz2l2sz21xv1xlo2l2v1xlo2l2hi21xv1xv1xhi21x_617 into H_bst_xsz2l2sz21xv1xlo2l2v1xlo2l2hi2v1xv1xhi2_617.
+try rename h_bst_xsz2l2sz21xv1xlo2l2v1xlo2l2hi2v1xv1xhi2_617 into h_bst_xsz2l2sz2v1xlo2l2v1xlo2l2hi2v1xv1xhi2_617.
+try rename H_bst_xsz2l2sz21xv1xlo2l2v1xlo2l2hi2v1xv1xhi2_617 into H_bst_xsz2l2sz2v1xlo2l2v1xlo2l2hi2v1xv1xhi2_617.
 ssl_write (l2 .+ 2).
 ssl_write_post (l2 .+ 2).
 ssl_write retv.
 ssl_write_post retv.
 ssl_write (x .+ 1).
 ssl_write_post (x .+ 1).
-try rename h_bst_xsz2l2sz2v1xlo2l2v1xlo2l2hi2v1xv1xhi2_528 into h_bst_xsz2l2sz2v2lo2l2v2lo2l2hi2v2v2hi2_528.
-try rename H_bst_xsz2l2sz2v1xlo2l2v1xlo2l2hi2v1xv1xhi2_528 into H_bst_xsz2l2sz2v2lo2l2v2lo2l2hi2v2v2hi2_528.
+try rename h_bst_xsz2l2sz2v1xlo2l2v1xlo2l2hi2v1xv1xhi2_617 into h_bst_xsz2l2sz2v2lo2l2v2lo2l2hi2v2v2hi2_617.
+try rename H_bst_xsz2l2sz2v1xlo2l2v1xlo2l2hi2v1xv1xhi2_617 into H_bst_xsz2l2sz2v2lo2l2v2lo2l2hi2v2v2hi2_617.
 ssl_emp;
 exists (sz1l2), (((1) + (sz2l2)) + (sz2)), (vl22), (hi1l2), ((if (v2) <= (lo2l2) then v2 else lo2l2)), (ll22), (lo1l2), ((if (hi2) <= (v2) then v2 else hi2)), (l2);
-exists (h_bst_ll22sz1l2lo1l2hi1l2_525l2);
-exists (x :-> v2 \+ x .+ 1 :-> rl22 \+ x .+ 2 :-> r2 \+ h_bst_rl22sz2l2lo2l2hi2l2_526l2 \+ h_bst_r2sz2lo2hi2_b);
+exists (h_bst_ll22sz1l2lo1l2hi1l2_614l2);
+exists (x :-> v2 \+ x .+ 1 :-> rl22 \+ x .+ 2 :-> r2 \+ h_bst_rl22sz2l2lo2l2hi2l2_615l2 \+ h_bst_r2sz2lo2hi2_b);
 sslauto.
 shelve.
-unfold_constructor 2;
-exists (sz2l2), (sz2), (v2), (hi2), (hi2l2), (lo2l2), (lo2), (rl22), (r2), (h_bst_rl22sz2l2lo2l2hi2l2_526l2), (h_bst_r2sz2lo2hi2_b);
+ssl_close 2;
+exists (sz2l2), (sz2), (v2), (hi2), (hi2l2), (lo2l2), (lo2), (rl22), (r2), (h_bst_rl22sz2l2lo2l2hi2l2_615l2), (h_bst_r2sz2lo2hi2_b);
 sslauto.
 shelve.
 shelve.
