lib/core.v
@@ -5,34 +5,21 @@ From fcsl
 Require Import prelude pred pcm unionmap heap.
 From HTT
 Require Import stmod stsep stlog stlogR.
-From Hammer Require Import Hammer.
+From Hammer Require Import Tactics.
 Require Import ZArith.
-
-(* Configure Hammer *)
-Unset Hammer Eprover.
-Unset Hammer Vampire.
-Add Search Blacklist "fcsl.".
-Add Search Blacklist "HTT.".
-Add Search Blacklist "Coq.ssr.ssrfun".
-Add Search Blacklist "mathcomp.ssreflect.ssrfun".
-Add Search Blacklist "mathcomp.ssreflect.bigop".
-Add Search Blacklist "mathcomp.ssreflect.choice".
-Add Search Blacklist "mathcomp.ssreflect.div".
-Add Search Blacklist "mathcomp.ssreflect.finfun".
-Add Search Blacklist "mathcomp.ssreflect.fintype".
-Add Search Blacklist "mathcomp.ssreflect.path".
-Add Search Blacklist "mathcomp.ssreflect.tuple".
 
 (* The empty heap *)
 Definition empty := @PCM.unit heapPCM.
 
 (* No-op at the end of a program branch *)
+
 Definition skip := ret tt.
 
 Inductive ltac_No_arg : Set :=
 | ltac_no_arg : ltac_No_arg.
 
 (* Utilities to move a heaplet around within a heap *)
+
 Ltac put_to_tail_ptr p :=
   try rewrite ptrA; rewrite -?joinA; rewrite ?(joinC (p :-> _) _); rewrite ?joinA.
 
@@ -47,23 +34,6 @@ Ltac put_to_head h :=
   put_to_tail h;
   try rewrite (joinC _ h).
 
-(* Utilities for nat and seq nat *)
-
-Ltac put_to_tail_nat n :=
-  rewrite -?addnA; rewrite ?(addnC n _); rewrite ?addnA.
-
-Ltac nat_add_eq' ns :=
-  match ns with
-  | ?A + ?B => put_to_tail_nat B; nat_add_eq' A
-  | ?A => put_to_tail A
-  end.
-
-Ltac nat_add_eq :=
-  by rewrite ?addnA;
-  match goal with
-  | [|- ?LHS = _] => nat_add_eq' LHS
-  end.
-
 (* Store heap validity assertions *)
 Ltac store_valid :=
   rewrite ?unitL ?unitR;
@@ -71,8 +41,7 @@ Ltac store_valid :=
   | [|- is_true (valid _) -> _] =>
     let hyp := fresh "H_valid" in move=>hyp;
     store_valid
-  end
-.
+  end.
 
 (* If goal is to prove a pointer is not null, derive that fact from one of the heap validity assertions *)
 Ltac assert_not_null :=
@@ -90,80 +59,6 @@ Ltac assert_not_null :=
     derive H x
   end.
 
-(* Theory about seq nats *)
-
-Create HintDb ssl_seqnat.
-
-Lemma subset_singleton (A : eqType) (s1: seq A) (x: A):
-  {subset s1 <= [::x]} -> {subset x :: s1 <= [::x]}.
-Proof.
-move=>H n.
-rewrite inE; move/orP. case.
-move/eqP=>->. by rewrite inE eqxx.
-move/H=>//.
-Qed.
-
-Lemma perm_eq_trans_el (A: eqType) (s1 s2 s3: seq A) (a b : A):
-  perm_eq s1 (a :: s2) ->
-  perm_eq s2 (b :: s3)->
-  perm_eq s1 [:: a, b & s3].
-Proof.
-move=> /permP H1 /permP H2; apply/permP=>n; move: (H1 n)  (H2 n) => //= -> -> //=.
-Qed.
-
-Lemma perm_eq_nil_r (A: eqType) (s: seq A): perm_eq s nil -> s = nil.
-Proof. by move/perm_nilP. Qed.
-
-Lemma perm_eq_nil_l (A: eqType) (s: seq A): perm_eq nil s -> s = nil.
-Proof. by rewrite perm_sym; move/perm_nilP. Qed.
-
-Hint Resolve subset_singleton : ssl_seqnat.
-Hint Resolve perm_eq_trans_el : ssl_seqnat.
-Hint Extern 1 (is_true (perm_eq _ _)) =>
-  match goal with
-  | [H: is_true (perm_eq _ nil) |- _] => apply perm_eq_nil_r in H; subst
-  | [H: is_true (perm_eq nil _) |- _] => apply perm_eq_nil_l in H; subst
-  end : ssl_seqnat.
-Hint Extern 1 (is_true (perm_eq _ _)) => apply/permP=>//=?; nat_add_eq : ssl_seqnat.
-
-Hint Rewrite <- cat_cons : ssl_seqnat.
-Hint Rewrite cat_cons : ssl_seqnat.
-Hint Rewrite perm_cat2r : ssl_seqnat.
-Lemma ssl_perm_sym (A: eqType) (x y: seq A): perm_eq x y -> perm_eq y x = perm_eq x y.
-Proof. by rewrite perm_sym. Qed.
-Hint Rewrite ssl_perm_sym using assumption: ssl_seqnat.
-
-Ltac solve_perm_eq :=
-  let n := fresh "n" in
-  apply/permP=>n;
-  repeat match goal with
-         | [H: is_true (perm_eq _ _) |- _] => move/permP in H; move:(H n)
-         end;
-  move=>//=;
-  rewrite ?count_cat;
-  zify; lia.
-
-(* Theory about nats *)
-
-Create HintDb ssl_nat.
-
-Lemma leq_neg (x y : nat) : (x <= y) = false -> y <= x.
-Proof. by case: ltngtP=>//. Qed.
-
-Hint Resolve leq_neg : ssl_nat.
-
-(* Theory about heaps *)
-
-Create HintDb ssl_heap.
-
-Ltac hhauto' h :=
-  match type of h with
-  | PCM.sort heapPCM => hhauto
-  | PCM.sort (union_map_classPCM heapUMC) => hhauto
-  end.
-
-Hint Extern 1 (?h = _) => hhauto' h : ssl_heap.
-
 (* Theory about predicates (to be filled by each certificate) *)
 
 Create HintDb ssl_pred.
@@ -179,16 +74,26 @@ Ltac eq_bool_to_prop :=
          | [H: is_true (_ == _) |- _] => move/eqP in H
          end.
 
+Ltac solve_perm_eq :=
+  let n := fresh "n" in
+  apply/permP=>n;
+  repeat match goal with
+         | [H: is_true (perm_eq _ _) |- _] => move/permP in H; move:(H n)
+         end;
+  move=>//=;
+  rewrite ?count_cat;
+  zify; lia.
+
+Ltac solve_pure := (timeout 2 progress eauto 2 with ssl_pure) + (sauto depth: 3).
+
 Ltac sslauto :=
   let simplify := eq_bool_to_prop; subst in
-  let sslauto_seqnat := (eauto with ssl_heap ssl_nat ssl_seqnat; autorewrite with ssl_seqnat=>//=) in
-  let solve_pure := (timeout 3 sauto) + (timeout 3 eauto 2 with ssl_pure) in
   repeat apply conj;
   match goal with
-  | [|- {subset _ <= _}] => sslauto_seqnat
+  | [|- {subset _ <= _}] => simplify; unshelve solve_pure; done
   | [|- is_true (perm_eq _ _)] => solve_perm_eq
-  | [|- _ = _] => simplify; rewrite ?unitL ?unitR; auto with ssl_heap ssl_nat
-  | [|- is_true (_ == _)] => simplify; unshelve (solve_pure + (apply/eqP; solve_pure)); done
+  | [|- _ = _] => simplify; rewrite ?unitL ?unitR; hhauto
+  | [|- is_true (_ == _)] => simplify; apply/eqP; unshelve solve_pure; done
   | [|- is_true (_ < _)] => simplify; unshelve solve_pure; done
   | [|- is_true (_ <= _)] => simplify; unshelve solve_pure; done
   | _ => idtac
@@ -211,20 +116,24 @@ Tactic Notation "ex_elim" ident(A) ident(B) ident(C) ident(D) ident(E) ident(F) 
 (***********)
 
 (* After binding program variables to their correct labels, we use the Coq's default simplification algorithm *)
+
 Ltac ssl_program_simpl := Tactics.program_simpl.
 
 
 (* Ghost Variable Elim *)
+
 Ltac ssl_ghostelim_pre := try apply: ghR; move=>h_self//=.
 
 Ltac ssl_ghostelim_post := store_valid.
 
 (* Read Rule *)
+
 Ltac ssl_read from :=
   put_to_head_ptr from;
   apply: bnd_readR=>/=.
 
 (* Write Rule *)
+
 Ltac ssl_write x :=
   put_to_head_ptr x; (* this significantly speeds up bnd_writeR *)
   apply: bnd_writeR=>/=.
@@ -233,10 +142,12 @@ Ltac ssl_write_post x :=
   (put_to_tail_ptr x + rewrite -(unitL (x :-> _))); apply frame.
 
 (* Alloc Rule *)
+
 Ltac ssl_alloc x :=
   apply: bnd_allocbR=>x//=.
 
 (* Free Rule *)
+
 Ltac ssl_dealloc x :=
   apply: bnd_seq;
   put_to_head_ptr x;
@@ -244,6 +155,7 @@ Ltac ssl_dealloc x :=
   rewrite ?unitR.
 
 (* Call Rule *)
+
 Ltac ssl_call_pre_aux h :=
   match h with
   | ?h1 \+ ?h2 => put_to_head h2; ssl_call_pre_aux h1
@@ -268,6 +180,7 @@ Tactic Notation "ssl_call" := ssl_call' ltac_No_arg.
 Tactic Notation "ssl_call" constr(ex) := ssl_call' ex.
 
 (* Emp Rule *)
+
 Ltac ssl_emp := apply: val_ret; rewrite ?unitL; store_valid; move=>//.
 
 (* Open Rule *)
@@ -294,41 +207,37 @@ Ltac ssl_open sel hyp :=
   case: hyp;
   (case: (ifP sel); try move/negbT; demorgan; move=>_//) + demorgan .
 
-(* Abduce Branch Rule *)
-Ltac ssl_abduce_branch sel :=
+(* Branch Rule *)
+
+Ltac ssl_branch sel :=
   let H := fresh "H_cond" in
   try case: (ifP sel);
   try move/negbT;
   try demorgan.
 
-(* Inconsistency *)
+(* Inconsistency Rule *)
+
 Ltac ssl_inconsistency :=
   match goal with
   | [H_true: is_true ?sel, H_false: is_true (~~ ?sel) |- _] => rewrite H_true in H_false=>//=
   end.
 
-(* Close *)
-Ltac unfold_constructor n :=
-  (*eauto with ssl_pred;*)
+(* Close Rule *)
+
+Ltac ssl_close n :=
+  match n with
+  | 1 => constructor 1=>//
+  | 2 => constructor 2=>//
+  | 3 => constructor 3=>//
+  | _ => constructor=>//
+  end;
   match goal with
-  (* There was nothing to solve; this happens if a preceding step *)
-  (* unwittingly solved the intended goal without needing to unfold. *)
-  | [|- verify _ _ _] =>
-    idtac
-  (* Unfold and discharge selector goal if needed *)
-  | _ => match n with
-         | 1 => constructor 1=>//
-         | 2 => constructor 2=>//
-         | 3 => constructor 3=>//
-         | _ => constructor=>//
-         end;
-         match goal with
-         | [|- is_true (_ != null)] => assert_not_null
-         | [|- (_ == null) = false] => apply negbTE; assert_not_null
-         | _ => idtac
-         end
+  | [|- is_true (_ != null)] => assert_not_null
+  | [|- (_ == null) = false] => apply negbTE; assert_not_null
+  | _ => idtac
   end.
 
-(* Frame Unfold *)
+(* Frame Unfold Rule *)
+
 Ltac ssl_frame_unfold :=
   (eq_bool_to_prop; subst; assumption) + (timeout 3 eauto 2 with ssl_pred).
